cleanq/crb: towawrds non-atomic pointer increases and space checks
Signed-off-by: Reto Achermann <reto.achermann@inf.ethz.ch>

CleanQ/CleanQ_CRBModel_Complx.thy
@@ -61,11 +61,17 @@ text \<open>
 (* Define some global variables to make Simpl/Complex proofs work *)
 record CleanQ_CRB_State_vars = 
   CRB  :: "CleanQ_Buffer CleanQ_RB_State"
+  CRB_prev  :: "CleanQ_Buffer CleanQ_RB_State"
   buf_x :: "CleanQ_Buffer"
   buf_y :: "CleanQ_Buffer"
-  local_x :: "CleanQ_Buffer"
-  local_y :: "CleanQ_Buffer"
   uni :: "CleanQ_Buffer set"
+  tail_x :: nat
+  tail_y :: nat
+  head_x :: nat
+  head_y :: nat
+  size_x :: nat
+  size_y :: nat
+
 (*>*)
 
 (* ------------------------------------------------------------------------------------ *)
@@ -79,6 +85,87 @@ text \<open>
   be represented as a sequence of atomic steps. We therefore define read and write 
   operations for buffer fields accordingly.  
 \<close>
+
+
+paragraph \<open>Reading the Pointers\<close>
+
+text \<open>
+  We need to make the access to the tail and head pointers explict. We do this by
+  providing this reading functions, which read the pointers in the ring.
+\<close>
+
+definition CleanQ_RB_read_tail_rx_x ::"'a CleanQ_RB_State \<Rightarrow> nat"
+  where "CleanQ_RB_read_tail_rx_x rb = tail (rTYX rb)"
+
+definition CleanQ_RB_read_tail_tx_x ::"'a CleanQ_RB_State \<Rightarrow> nat"
+  where "CleanQ_RB_read_tail_tx_x rb = tail (rTXY rb)"
+
+definition CleanQ_RB_read_tail_rx_y ::"'a CleanQ_RB_State \<Rightarrow> nat"
+  where "CleanQ_RB_read_tail_rx_y rb = tail (rTXY rb)"
+
+definition CleanQ_RB_read_tail_tx_y ::"'a CleanQ_RB_State \<Rightarrow> nat"
+  where "CleanQ_RB_read_tail_tx_y rb = tail (rTYX rb)"
+
+definition CleanQ_RB_read_head_rx_x ::"'a CleanQ_RB_State \<Rightarrow> nat"
+  where "CleanQ_RB_read_head_rx_x rb = head (rTYX rb)"
+
+definition CleanQ_RB_read_head_tx_x ::"'a CleanQ_RB_State \<Rightarrow> nat"
+  where "CleanQ_RB_read_head_tx_x rb = head (rTXY rb)"
+
+definition CleanQ_RB_read_head_rx_y ::"'a CleanQ_RB_State \<Rightarrow> nat"
+  where "CleanQ_RB_read_head_rx_y rb = head (rTXY rb)"
+
+definition CleanQ_RB_read_head_tx_y ::"'a CleanQ_RB_State \<Rightarrow> nat"
+  where "CleanQ_RB_read_head_tx_y rb = head (rTYX rb)"
+
+definition CleanQ_RB_read_size_rx_x ::"'a CleanQ_RB_State \<Rightarrow> nat"
+  where "CleanQ_RB_read_size_rx_x rb = size (rTYX rb)"
+
+definition CleanQ_RB_read_size_tx_x ::"'a CleanQ_RB_State \<Rightarrow> nat"
+  where "CleanQ_RB_read_size_tx_x rb = size (rTXY rb)"
+
+definition CleanQ_RB_read_size_rx_y ::"'a CleanQ_RB_State \<Rightarrow> nat"
+  where "CleanQ_RB_read_size_rx_y rb = size (rTXY rb)"
+
+definition CleanQ_RB_read_size_tx_y ::"'a CleanQ_RB_State \<Rightarrow> nat"
+  where "CleanQ_RB_read_size_tx_y rb = size (rTYX rb)"
+
+text \<open>
+  They are equivalent over cross i.e. rx_x = tx_y
+\<close>
+
+lemma "CleanQ_RB_read_tail_rx_x rb = CleanQ_RB_read_tail_tx_y rb"
+  unfolding CleanQ_RB_read_tail_rx_x_def CleanQ_RB_read_tail_tx_y_def by auto
+
+lemma "CleanQ_RB_read_tail_tx_x rb = CleanQ_RB_read_tail_rx_y rb"
+  unfolding CleanQ_RB_read_tail_tx_x_def CleanQ_RB_read_tail_rx_y_def by auto
+
+lemma "CleanQ_RB_read_head_rx_x rb = CleanQ_RB_read_head_tx_y rb"
+  unfolding CleanQ_RB_read_head_rx_x_def CleanQ_RB_read_head_tx_y_def by auto
+
+lemma "CleanQ_RB_read_head_tx_x rb = CleanQ_RB_read_head_rx_y rb"
+  unfolding CleanQ_RB_read_head_tx_x_def CleanQ_RB_read_head_rx_y_def by auto
+
+lemma "CleanQ_RB_read_size_rx_x rb = CleanQ_RB_read_size_tx_y rb"
+  unfolding CleanQ_RB_read_size_rx_x_def CleanQ_RB_read_size_tx_y_def by auto
+
+lemma "CleanQ_RB_read_size_tx_x rb = CleanQ_RB_read_size_rx_y rb"
+  unfolding CleanQ_RB_read_size_tx_x_def CleanQ_RB_read_size_rx_y_def by auto
+
+paragraph \<open>Writing the Pointers\<close>
+
+definition CleanQ_RB_write_headptr_x :: "nat \<Rightarrow> 'a CleanQ_RB_State \<Rightarrow> 'a CleanQ_RB_State"
+  where "CleanQ_RB_write_headptr_x v rb = rb \<lparr> rTXY := (rTXY rb) \<lparr> head := v \<rparr> \<rparr>"
+
+definition CleanQ_RB_write_headptr_y :: "nat \<Rightarrow> 'a CleanQ_RB_State \<Rightarrow> 'a CleanQ_RB_State"
+  where "CleanQ_RB_write_headptr_y v rb = rb \<lparr> rTYX := (rTYX rb) \<lparr> head := v \<rparr> \<rparr>"
+
+definition CleanQ_RB_write_tailptr_x :: "nat \<Rightarrow> 'a CleanQ_RB_State \<Rightarrow> 'a CleanQ_RB_State"
+  where "CleanQ_RB_write_tailptr_x v rb = rb \<lparr> rTYX := (rTYX rb) \<lparr> tail := v \<rparr> \<rparr>"
+
+definition CleanQ_RB_write_tailptr_y :: "nat \<Rightarrow> 'a CleanQ_RB_State \<Rightarrow> 'a CleanQ_RB_State"
+  where "CleanQ_RB_write_tailptr_y v rb = rb \<lparr> rTXY := (rTXY rb) \<lparr> tail := v \<rparr> \<rparr>"
+
 
 paragraph \<open>Reading a Buffer\<close>
 
@@ -595,12 +682,17 @@ lemma CleanQ_RB_write_head_valid_length_x_read_x_length_unchanged:
       = length (CleanQ_RB_read_head_x rb)"
   by (simp add: CleanQ_RB_read_head_x_def CleanQ_RB_write_head_valid_length_x_def)
 
+lemma CleanQ_RB_write_head_length_x_eq :
+  "length (CleanQ_RB_read_head_x (CleanQ_RB_write_head_length_x b rb)) = length b"
+  by (simp add: CleanQ_RB_read_head_x_def CleanQ_RB_write_head_length_x_def)
+
 lemmas CleanQ_RB_write_head_x_read_x_length_unchanged_simps[simp] = 
     CleanQ_RB_write_head_offset_x_read_x_length_unchanged
     CleanQ_RB_write_head_region_x_read_x_length_unchanged
     CleanQ_RB_write_head_flags_x_read_x_length_unchanged
     CleanQ_RB_write_head_valid_offset_x_read_x_length_unchanged
     CleanQ_RB_write_head_valid_length_x_read_x_length_unchanged
+    CleanQ_RB_write_head_length_x_eq
 
 
 paragraph \<open>Length Head Y Unchanged, Update Other Fields Head X\<close>
@@ -665,12 +757,17 @@ lemma CleanQ_RB_write_head_valid_length_y_read_y_length_unchanged:
       = length (CleanQ_RB_read_head_y rb)"
   by (simp add: CleanQ_RB_read_head_y_def CleanQ_RB_write_head_valid_length_y_def)
 
+lemma CleanQ_RB_write_head_length_y_eq :
+  "length (CleanQ_RB_read_head_y (CleanQ_RB_write_head_length_y b rb)) = length b"
+  by (simp add: CleanQ_RB_read_head_y_def CleanQ_RB_write_head_length_y_def)
+
 lemmas CleanQ_RB_write_head_y_read_y_length_unchanged_simps[simp] = 
     CleanQ_RB_write_head_offset_y_read_y_length_unchanged
     CleanQ_RB_write_head_region_y_read_y_length_unchanged
     CleanQ_RB_write_head_flags_y_read_y_length_unchanged
     CleanQ_RB_write_head_valid_offset_y_read_y_length_unchanged
     CleanQ_RB_write_head_valid_length_y_read_y_length_unchanged
+    CleanQ_RB_write_head_length_y_eq
 
 
 paragraph \<open>Length Head X Unchanged, Update Other Fields Head Y\<close>
@@ -734,13 +831,18 @@ lemma CleanQ_RB_write_head_valid_length_x_read_x_offset_unchanged:
   "offset (CleanQ_RB_read_head_x (CleanQ_RB_write_head_valid_length_x x rb)) 
     = offset (CleanQ_RB_read_head_x rb)"
   by (simp add: CleanQ_RB_read_head_x_def CleanQ_RB_write_head_valid_length_x_def)
- 
+
+lemma CleanQ_RB_write_head_offset_x_eq :
+  "offset (CleanQ_RB_read_head_x (CleanQ_RB_write_head_offset_x b rb)) = offset b"
+  by (simp add: CleanQ_RB_read_head_x_def CleanQ_RB_write_head_offset_x_def)
+
 lemmas CleanQ_RB_write_head_x_read_x_offset_unchanged_simps[simp] = 
     CleanQ_RB_write_head_length_x_read_x_offset_unchanged
     CleanQ_RB_write_head_region_x_read_x_offset_unchanged
     CleanQ_RB_write_head_flags_x_read_x_offset_unchanged
     CleanQ_RB_write_head_valid_offset_x_read_x_offset_unchanged
     CleanQ_RB_write_head_valid_length_x_read_x_offset_unchanged
+    CleanQ_RB_write_head_offset_x_eq
 
 
 paragraph \<open>Offset Head Y Unchanged, Update Other Fields Head X\<close>
@@ -805,12 +907,17 @@ lemma CleanQ_RB_write_head_valid_length_y_read_y_offset_unchanged:
       = offset (CleanQ_RB_read_head_y rb)"
   by (simp add: CleanQ_RB_read_head_y_def CleanQ_RB_write_head_valid_length_y_def)
 
+lemma CleanQ_RB_write_head_offset_y_eq :
+  "offset (CleanQ_RB_read_head_y (CleanQ_RB_write_head_offset_y b rb)) = offset b"
+  by (simp add: CleanQ_RB_read_head_y_def CleanQ_RB_write_head_offset_y_def)
+
 lemmas CleanQ_RB_write_head_y_read_y_offset_unchanged_simps[simp] = 
     CleanQ_RB_write_head_length_y_read_y_offset_unchanged
     CleanQ_RB_write_head_region_y_read_y_offset_unchanged
     CleanQ_RB_write_head_flags_y_read_y_offset_unchanged
     CleanQ_RB_write_head_valid_offset_y_read_y_offset_unchanged
     CleanQ_RB_write_head_valid_length_y_read_y_offset_unchanged
+    CleanQ_RB_write_head_offset_y_eq
 
 
 paragraph \<open>Offset Head X Unchanged, Update Other Fields Head Y\<close>
@@ -874,13 +981,18 @@ lemma CleanQ_RB_write_head_valid_length_x_read_x_flags_unchanged:
   "flags (CleanQ_RB_read_head_x (CleanQ_RB_write_head_valid_length_x x rb)) 
     = flags (CleanQ_RB_read_head_x rb)"
   by (simp add: CleanQ_RB_read_head_x_def CleanQ_RB_write_head_valid_length_x_def)
-  
+
+lemma CleanQ_RB_write_head_flags_x_eq :
+  "flags (CleanQ_RB_read_head_x (CleanQ_RB_write_head_flags_x b rb)) = flags b"
+  by (simp add: CleanQ_RB_read_head_x_def CleanQ_RB_write_head_flags_x_def)
+
 lemmas CleanQ_RB_write_head_x_read_x_flags_unchanged_simps[simp] = 
     CleanQ_RB_write_head_length_x_read_x_flags_unchanged
     CleanQ_RB_write_head_region_x_read_x_flags_unchanged
     CleanQ_RB_write_head_offset_x_read_x_flags_unchanged
     CleanQ_RB_write_head_valid_offset_x_read_x_flags_unchanged
     CleanQ_RB_write_head_valid_length_x_read_x_flags_unchanged
+    CleanQ_RB_write_head_flags_x_eq
 
 paragraph \<open>Flags Head Y Unchanged, Update Other Fields Head X\<close>
 
@@ -944,12 +1056,17 @@ lemma CleanQ_RB_write_head_valid_length_y_read_y_flags_unchanged:
     = flags (CleanQ_RB_read_head_y rb)"
   by (simp add: CleanQ_RB_read_head_y_def CleanQ_RB_write_head_valid_length_y_def)
 
+lemma CleanQ_RB_write_head_flags_y_eq :
+  "flags (CleanQ_RB_read_head_y (CleanQ_RB_write_head_flags_y b rb)) = flags b"
+  by (simp add: CleanQ_RB_read_head_y_def CleanQ_RB_write_head_flags_y_def)
+
 lemmas CleanQ_RB_write_head_y_read_y_flags_unchanged_simps[simp] = 
     CleanQ_RB_write_head_length_y_read_y_flags_unchanged
     CleanQ_RB_write_head_region_y_read_y_flags_unchanged
     CleanQ_RB_write_head_offset_y_read_y_flags_unchanged
     CleanQ_RB_write_head_valid_offset_y_read_y_flags_unchanged
     CleanQ_RB_write_head_valid_length_y_read_y_flags_unchanged
+    CleanQ_RB_write_head_flags_y_eq
 
 
 paragraph \<open>Flags Head X Unchanged, Update Other Fields Head Y\<close>
@@ -1013,13 +1130,18 @@ lemma CleanQ_RB_write_head_valid_length_x_read_x_region_unchanged:
   "region (CleanQ_RB_read_head_x (CleanQ_RB_write_head_valid_length_x x rb)) 
     = region (CleanQ_RB_read_head_x rb)"
   by (simp add: CleanQ_RB_read_head_x_def CleanQ_RB_write_head_valid_length_x_def)
-  
+
+lemma CleanQ_RB_write_head_region_x_eq :
+  "region (CleanQ_RB_read_head_x (CleanQ_RB_write_head_region_x b rb)) = region b"
+  by (simp add: CleanQ_RB_read_head_x_def CleanQ_RB_write_head_region_x_def)
+
 lemmas CleanQ_RB_write_head_x_read_x_region_unchanged_simps[simp] = 
     CleanQ_RB_write_head_length_x_read_x_region_unchanged
     CleanQ_RB_write_head_flags_x_read_x_region_unchanged
     CleanQ_RB_write_head_offset_x_read_x_region_unchanged
     CleanQ_RB_write_head_valid_offset_x_read_x_region_unchanged
     CleanQ_RB_write_head_valid_length_x_read_x_region_unchanged
+    CleanQ_RB_write_head_region_x_eq
 
 
 paragraph \<open>Region Head Y Unchanged, Update Other Fields Head X\<close>
@@ -1084,12 +1206,17 @@ lemma CleanQ_RB_write_head_valid_length_y_read_y_region_unchanged:
     = region (CleanQ_RB_read_head_y rb)"
   by (simp add: CleanQ_RB_read_head_y_def CleanQ_RB_write_head_valid_length_y_def)
 
+lemma CleanQ_RB_write_head_region_y_eq :
+  "region (CleanQ_RB_read_head_y (CleanQ_RB_write_head_region_y b rb)) = region b"
+  by (simp add: CleanQ_RB_read_head_y_def CleanQ_RB_write_head_region_y_def)
+
 lemmas CleanQ_RB_write_head_y_read_y_region_unchanged_simps[simp] = 
     CleanQ_RB_write_head_length_y_read_y_region_unchanged
     CleanQ_RB_write_head_flags_y_read_y_region_unchanged
     CleanQ_RB_write_head_offset_y_read_y_region_unchanged
     CleanQ_RB_write_head_valid_offset_y_read_y_region_unchanged
     CleanQ_RB_write_head_valid_length_y_read_y_region_unchanged
+    CleanQ_RB_write_head_region_y_eq
 
 
 paragraph \<open>Region Head X Unchanged, Update Other Fields Head Y\<close>
@@ -1153,13 +1280,19 @@ lemma CleanQ_RB_write_head_valid_length_x_read_x_valid_offset_unchanged:
   "valid_offset (CleanQ_RB_read_head_x (CleanQ_RB_write_head_valid_length_x x rb)) 
     = valid_offset (CleanQ_RB_read_head_x rb)"
   by (simp add: CleanQ_RB_read_head_x_def CleanQ_RB_write_head_valid_length_x_def)
- 
+
+lemma CleanQ_RB_write_head_valid_offset_x_eq :
+  "valid_offset (CleanQ_RB_read_head_x (CleanQ_RB_write_head_valid_offset_x b rb)) 
+      = valid_offset b"
+  by (simp add: CleanQ_RB_read_head_x_def CleanQ_RB_write_head_valid_offset_x_def)
+
 lemmas CleanQ_RB_write_head_x_read_x_valid_offset_unchanged_simps[simp] = 
     CleanQ_RB_write_head_length_x_read_x_valid_offset_unchanged
     CleanQ_RB_write_head_flags_x_read_x_valid_offset_unchanged
     CleanQ_RB_write_head_offset_x_read_x_valid_offset_unchanged
     CleanQ_RB_write_head_region_x_read_x_valid_offset_unchanged
     CleanQ_RB_write_head_valid_length_x_read_x_valid_offset_unchanged
+    CleanQ_RB_write_head_valid_offset_x_eq
 
 
 paragraph \<open>Valid Offset Head Y Unchanged, Update Other Fields Head X\<close>
@@ -1224,12 +1357,18 @@ lemma CleanQ_RB_write_head_valid_length_y_read_y_valid_offset_unchanged:
     = valid_offset (CleanQ_RB_read_head_y rb)"
   by (simp add: CleanQ_RB_read_head_y_def CleanQ_RB_write_head_valid_length_y_def)
 
+lemma CleanQ_RB_write_head_valid_offset_y_eq :
+  "valid_offset (CleanQ_RB_read_head_y (CleanQ_RB_write_head_valid_offset_y b rb)) 
+       = valid_offset b"
+  by (simp add: CleanQ_RB_read_head_y_def CleanQ_RB_write_head_valid_offset_y_def)
+
 lemmas CleanQ_RB_write_head_y_read_y_valid_offset_unchanged_simps[simp] = 
     CleanQ_RB_write_head_length_y_read_y_valid_offset_unchanged
     CleanQ_RB_write_head_flags_y_read_y_valid_offset_unchanged
     CleanQ_RB_write_head_offset_y_read_y_valid_offset_unchanged
     CleanQ_RB_write_head_region_y_read_y_valid_offset_unchanged
     CleanQ_RB_write_head_valid_length_y_read_y_valid_offset_unchanged
+    CleanQ_RB_write_head_valid_offset_y_eq
 
 
 paragraph \<open>Valid Offset Head X Unchanged, Update Other Fields Head Y\<close>
@@ -1294,12 +1433,18 @@ lemma CleanQ_RB_write_head_valid_offset_x_read_x_valid_length_unchanged:
     = valid_length (CleanQ_RB_read_head_x rb)"
   by (simp add: CleanQ_RB_read_head_x_def CleanQ_RB_write_head_valid_offset_x_def)
 
+lemma CleanQ_RB_write_head_valid_length_x_eq :
+  "valid_length (CleanQ_RB_read_head_x (CleanQ_RB_write_head_valid_length_x b rb)) 
+        = valid_length b"
+  by (simp add: CleanQ_RB_read_head_x_def CleanQ_RB_write_head_valid_length_x_def)
+
 lemmas CleanQ_RB_write_head_x_read_x_valid_length_unchanged_simps[simp] = 
     CleanQ_RB_write_head_length_x_read_x_valid_length_unchanged
     CleanQ_RB_write_head_flags_x_read_x_valid_length_unchanged
     CleanQ_RB_write_head_offset_x_read_x_valid_length_unchanged
     CleanQ_RB_write_head_region_x_read_x_valid_length_unchanged
     CleanQ_RB_write_head_valid_offset_x_read_x_valid_length_unchanged
+    CleanQ_RB_write_head_valid_length_x_eq
 
 
 paragraph \<open>Valid Length Head Y Unchanged, Update Other Fields Head X\<close>
@@ -1364,12 +1509,18 @@ lemma CleanQ_RB_write_head_valid_offset_y_read_y_valid_length_unchanged:
     = valid_length (CleanQ_RB_read_head_y rb)"
   by (simp add: CleanQ_RB_read_head_y_def CleanQ_RB_write_head_valid_offset_y_def)
 
+lemma CleanQ_RB_write_head_valid_length_y_eq :
+  "valid_length (CleanQ_RB_read_head_y (CleanQ_RB_write_head_valid_length_y b rb)) 
+      = valid_length b"
+  by (simp add: CleanQ_RB_read_head_y_def CleanQ_RB_write_head_valid_length_y_def)
+
 lemmas CleanQ_RB_write_head_y_read_y_valid_length_unchanged_simps[simp] = 
     CleanQ_RB_write_head_length_y_read_y_valid_length_unchanged
     CleanQ_RB_write_head_flags_y_read_y_valid_length_unchanged
     CleanQ_RB_write_head_offset_y_read_y_valid_length_unchanged
     CleanQ_RB_write_head_region_y_read_y_valid_length_unchanged
     CleanQ_RB_write_head_valid_offset_y_read_y_valid_length_unchanged
+    CleanQ_RB_write_head_valid_length_y_eq
 
 
 paragraph \<open>Valid Length Head X Unchanged, Update Other Fields Head Y\<close>
@@ -2105,6 +2256,19 @@ lemmas CleanQ_RB_write_head_y_SY_unchanged[simp] =
   CleanQ_RB_write_head_valid_offset_y_SY_unchanged
   CleanQ_RB_write_head_valid_length_y_SY_unchanged
 
+paragraph\<open>Enqueue head pointer nont in SX/SYS\<close>
+
+lemma CleanQ_RB_read_head_y_not_in_SY:
+  "CleanQ_RB_read_head_y rb \<notin> rSY (CleanQ_RB_enq_y (CleanQ_RB_read_head_y rb) rb)"
+  by(simp add: CleanQ_RB_enq_y_def) 
+
+lemma CleanQ_RB_read_head_x_not_in_SX:
+  "CleanQ_RB_read_head_x rb \<notin> rSX (CleanQ_RB_enq_x (CleanQ_RB_read_head_x rb) rb)"
+  by(simp add: CleanQ_RB_enq_x_def) 
+
+lemmas CleanQ_RB_read_head_y_not_in_S[simp] =
+  CleanQ_RB_read_head_y_not_in_SY
+  CleanQ_RB_read_head_x_not_in_SX
 
 (* ------------------------------------------------------------------------------------ *)
 subsubsection \<open>Nested Reading of Tail Element\<close>
@@ -3787,357 +3951,152 @@ lemmas CleanQ_RB_write_head_y_not_none[simp] =
 
 
 (* ------------------------------------------------------------------------------------ *)
-subsubsection \<open>TODO: Sort here\<close>
+subsubsection \<open>Reading All Fields is Reading Record\<close>
 (* ------------------------------------------------------------------------------------ *)
 
-paragraph \<open>Write head behaves as expected for X\<close>
+text \<open>
+  Finally, if all fields have been read in the process, then reading the last field
+  (i.e. the flags is equivalent to reading the entire record. Note this depends on
+  the flags being read last. 
+\<close>
 
-lemma CleanQ_RB_write_head_flags_x_eq:
-  assumes reg: "region (CleanQ_RB_read_head_x (CRB x)) = region b2" and
-          off: "offset (CleanQ_RB_read_head_x (CRB x)) = offset b2 " and
-          len: "length (CleanQ_RB_read_head_x (CRB x)) = length b2" and
-          vao: "valid_offset (CleanQ_RB_read_head_x (CRB x)) = valid_offset b2" and
-          val:"valid_length (CleanQ_RB_read_head_x (CRB x)) = valid_length b2"
-  shows "b2 = CleanQ_RB_read_head_x (CleanQ_RB_write_head_flags_x ( b2) (CRB x))"
-  using assms unfolding CleanQ_RB_write_head_flags_x_def CleanQ_RB_read_head_x_def
-  by(auto)
+lemma CleanQ_RB_read_tail_y_region:
+  "b = CleanQ_RB_read_tail_flags_y rb (b) \<Longrightarrow> b = CleanQ_RB_read_tail_offset_y rb (b) 
+    \<Longrightarrow> b = CleanQ_RB_read_tail_length_y rb (b) 
+    \<Longrightarrow> b = CleanQ_RB_read_tail_valid_offset_y rb (b) 
+    \<Longrightarrow> b = CleanQ_RB_read_tail_valid_length_y rb (b) \<Longrightarrow> 
+      CleanQ_RB_read_tail_region_y rb (b) = CleanQ_RB_read_tail_y rb"
+  by (metis CleanQ_RB_read_tail_flags_y_region_y CleanQ_RB_read_tail_length_y_region_y 
+            CleanQ_RB_read_tail_offset_y_region_y CleanQ_RB_read_tail_valid_length_y_region_y 
+            CleanQ_RB_read_tail_valid_offset_y_region_y CleanQ_RB_read_tail_y_fields_eq)
 
-lemma CleanQ_RB_write_head_region_x_eq :
-  shows "region (CleanQ_RB_read_head_x (CleanQ_RB_write_head_region_x ( b2) (CRB x))) = region b2"
-  by (simp add: CleanQ_RB_read_head_x_def CleanQ_RB_write_head_region_x_def)
+lemma CleanQ_RB_read_tail_y_offset:
+  "b = CleanQ_RB_read_tail_region_y rb (b) \<Longrightarrow> b = CleanQ_RB_read_tail_flags_y rb (b) 
+    \<Longrightarrow> b = CleanQ_RB_read_tail_length_y rb (b) 
+    \<Longrightarrow> b = CleanQ_RB_read_tail_valid_offset_y rb (b) 
+    \<Longrightarrow> b = CleanQ_RB_read_tail_valid_length_y rb (b) \<Longrightarrow> 
+      CleanQ_RB_read_tail_offset_y rb (b) = CleanQ_RB_read_tail_y rb"
+  by (metis CleanQ_RB_read_tail_flags_y_offset_y CleanQ_RB_read_tail_length_y_offset_y 
+            CleanQ_RB_read_tail_valid_length_y_offset_y CleanQ_RB_read_tail_valid_offset_y_offset_y 
+             CleanQ_RB_read_tail_y_fields_eq)
 
-lemma CleanQ_RB_write_head_offset_x_eq :
-  shows "offset (CleanQ_RB_read_head_x (CleanQ_RB_write_head_offset_x ( b2) (CRB x))) = offset b2"
-  by (simp add: CleanQ_RB_read_head_x_def CleanQ_RB_write_head_offset_x_def)
+lemma CleanQ_RB_read_tail_y_length:
+  "b = CleanQ_RB_read_tail_region_y rb (b) \<Longrightarrow> b = CleanQ_RB_read_tail_offset_y rb (b) 
+    \<Longrightarrow> b = CleanQ_RB_read_tail_flags_y rb (b) 
+    \<Longrightarrow> b = CleanQ_RB_read_tail_valid_offset_y rb (b) 
+    \<Longrightarrow> b = CleanQ_RB_read_tail_valid_length_y rb (b) \<Longrightarrow> 
+      CleanQ_RB_read_tail_length_y rb (b) = CleanQ_RB_read_tail_y rb"
+  by (metis CleanQ_RB_read_tail_flags_y_length_y CleanQ_RB_read_tail_valid_length_y_length_y
+            CleanQ_RB_read_tail_valid_offset_y_length_y CleanQ_RB_read_tail_y_fields_eq)
 
-lemma CleanQ_RB_write_head_length_x_eq :
-  shows "length (CleanQ_RB_read_head_x (CleanQ_RB_write_head_length_x ( b2) (CRB x))) = length b2"
-  by (simp add: CleanQ_RB_read_head_x_def CleanQ_RB_write_head_length_x_def)
+lemma CleanQ_RB_read_tail_y_valid_offset:
+  "b = CleanQ_RB_read_tail_region_y rb (b) \<Longrightarrow> b = CleanQ_RB_read_tail_offset_y rb (b) 
+    \<Longrightarrow> b = CleanQ_RB_read_tail_length_y rb (b) 
+    \<Longrightarrow> b = CleanQ_RB_read_tail_flags_y rb (b) 
+    \<Longrightarrow> b = CleanQ_RB_read_tail_valid_length_y rb (b) \<Longrightarrow> 
+      CleanQ_RB_read_tail_valid_offset_y rb (b) = CleanQ_RB_read_tail_y rb"
+  by (metis CleanQ_RB_read_tail_y_fields_eq)
 
-lemma CleanQ_RB_write_head_valid_length_x_eq :
-  shows "valid_length (CleanQ_RB_read_head_x (CleanQ_RB_write_head_valid_length_x ( b2) (CRB x))) = valid_length b2"
-  by (simp add: CleanQ_RB_read_head_x_def CleanQ_RB_write_head_valid_length_x_def)
-  
+lemma CleanQ_RB_read_tail_y_valid_length:
+  "b = CleanQ_RB_read_tail_region_y rb (b) \<Longrightarrow> b = CleanQ_RB_read_tail_offset_y rb (b) 
+    \<Longrightarrow> b = CleanQ_RB_read_tail_length_y rb (b) 
+    \<Longrightarrow> b = CleanQ_RB_read_tail_valid_offset_y rb (b) 
+    \<Longrightarrow> b = CleanQ_RB_read_tail_flags_y rb (b) \<Longrightarrow> 
+      CleanQ_RB_read_tail_valid_length_y rb (b) = CleanQ_RB_read_tail_y rb"
+  by (metis CleanQ_RB_read_tail_valid_offset_y_valid_length_y CleanQ_RB_read_tail_y_fields_eq)
 
-lemma CleanQ_RB_write_head_valid_offset_x_eq :
-  shows "valid_offset (CleanQ_RB_read_head_x (CleanQ_RB_write_head_valid_offset_x ( b2) (CRB x))) = valid_offset b2"
-  by (simp add: CleanQ_RB_read_head_x_def CleanQ_RB_write_head_valid_offset_x_def)
-  
-lemmas CleanQ_RB_write_head_x_eq[simp] = 
-  CleanQ_RB_write_head_region_x_eq
-  CleanQ_RB_write_head_offset_x_eq 
-  CleanQ_RB_write_head_length_x_eq
-  CleanQ_RB_write_head_valid_offset_x_eq
-  CleanQ_RB_write_head_valid_length_x_eq
-  CleanQ_RB_write_head_flags_x_eq
+lemma CleanQ_RB_read_tail_y_flags[simp]:
+  "b = CleanQ_RB_read_tail_region_y rb (b) \<Longrightarrow> b = CleanQ_RB_read_tail_offset_y rb (b) 
+    \<Longrightarrow> b = CleanQ_RB_read_tail_length_y rb (b) 
+    \<Longrightarrow> b = CleanQ_RB_read_tail_valid_offset_y rb (b) 
+    \<Longrightarrow> b = CleanQ_RB_read_tail_valid_length_y rb (b) \<Longrightarrow> 
+      CleanQ_RB_read_tail_flags_y rb (b) = CleanQ_RB_read_tail_y rb"
+  by (metis CleanQ_RB_read_tail_valid_length_y_flags_y CleanQ_RB_read_tail_valid_offset_y_flags_y 
+            CleanQ_RB_read_tail_y_fields_eq)
 
-paragraph \<open>Write head behaves as expected for Y\<close>
-
-lemma CleanQ_RB_write_head_flags_y_eq:
-  assumes reg: "region (CleanQ_RB_read_head_y (CRB x)) = region b2" and
-          off: "offset (CleanQ_RB_read_head_y (CRB x)) = offset b2 " and
-          len: "length (CleanQ_RB_read_head_y (CRB x)) = length b2" and
-          vao: "valid_offset (CleanQ_RB_read_head_y (CRB x)) = valid_offset b2" and
-          val:"valid_length (CleanQ_RB_read_head_y (CRB x)) = valid_length b2"
-  shows "b2 = CleanQ_RB_read_head_y (CleanQ_RB_write_head_flags_y ( b2) (CRB x))"
-  using assms unfolding CleanQ_RB_write_head_flags_y_def CleanQ_RB_read_head_y_def
-  by(auto)
-
-lemma CleanQ_RB_write_head_region_y_eq :
-  shows "region (CleanQ_RB_read_head_y (CleanQ_RB_write_head_region_y ( b2) (CRB y))) = region b2"
-  by (simp add: CleanQ_RB_read_head_y_def CleanQ_RB_write_head_region_y_def)
-
-lemma CleanQ_RB_write_head_offset_y_eq :
-  shows "offset (CleanQ_RB_read_head_y (CleanQ_RB_write_head_offset_y ( b2) (CRB y))) = offset b2"
-  by (simp add: CleanQ_RB_read_head_y_def CleanQ_RB_write_head_offset_y_def)
-
-lemma CleanQ_RB_write_head_length_y_eq :
-  shows "length (CleanQ_RB_read_head_y (CleanQ_RB_write_head_length_y ( b2) (CRB y))) = length b2"
-  by (simp add: CleanQ_RB_read_head_y_def CleanQ_RB_write_head_length_y_def)
-
-lemma CleanQ_RB_write_head_valid_length_y_eq :
-  shows "valid_length (CleanQ_RB_read_head_y (CleanQ_RB_write_head_valid_length_y ( b2) (CRB y))) = valid_length b2"
-  by (simp add: CleanQ_RB_read_head_y_def CleanQ_RB_write_head_valid_length_y_def)
-  
-lemma CleanQ_RB_write_head_valid_offset_y_eq :
-  shows "valid_offset (CleanQ_RB_read_head_y (CleanQ_RB_write_head_valid_offset_y ( b2) (CRB y))) = valid_offset b2"
-  by (simp add: CleanQ_RB_read_head_y_def CleanQ_RB_write_head_valid_offset_y_def)
-
-lemmas CleanQ_RB_write_head_y_eq[simp] = 
-  CleanQ_RB_write_head_region_y_eq
-  CleanQ_RB_write_head_offset_y_eq 
-  CleanQ_RB_write_head_length_y_eq
-  CleanQ_RB_write_head_valid_offset_y_eq
-  CleanQ_RB_write_head_valid_length_y_eq
-  CleanQ_RB_write_head_flags_y_eq
+lemmas CleanQ_RB_read_tail_y_fields_simp = 
+  CleanQ_RB_read_tail_y_region
+  CleanQ_RB_read_tail_y_offset
+  CleanQ_RB_read_tail_y_length
+  CleanQ_RB_read_tail_y_valid_offset
+  CleanQ_RB_read_tail_y_valid_length
+  CleanQ_RB_read_tail_y_flags
 
 
+lemma CleanQ_RB_read_tail_x_region:
+  "b = CleanQ_RB_read_tail_flags_x rb (b) \<Longrightarrow> b = CleanQ_RB_read_tail_offset_x rb (b) 
+    \<Longrightarrow> b = CleanQ_RB_read_tail_length_x rb (b) 
+    \<Longrightarrow> b = CleanQ_RB_read_tail_valid_offset_x rb (b) 
+    \<Longrightarrow> b = CleanQ_RB_read_tail_valid_length_x rb (b) \<Longrightarrow> 
+      CleanQ_RB_read_tail_region_x rb (b) = CleanQ_RB_read_tail_x rb"
+  by (metis CleanQ_RB_read_tail_flags_x_region_x CleanQ_RB_read_tail_length_x_region_x 
+            CleanQ_RB_read_tail_offset_x_region_x CleanQ_RB_read_tail_valid_length_x_region_x 
+            CleanQ_RB_read_tail_valid_offset_x_region_x CleanQ_RB_read_tail_x_fields_eq)
 
-lemma CleanQ_RB_read_tail_y_flags [simp]:
-  assumes "buf_y x = CleanQ_RB_read_tail_region_y (CRB x) (buf_y x)" and
-          "buf_y x = CleanQ_RB_read_tail_offset_y (CRB x) (buf_y x)" and
-          "buf_y x = CleanQ_RB_read_tail_length_y (CRB x) (buf_y x)" and
-          "buf_y x = CleanQ_RB_read_tail_valid_offset_y (CRB x) (buf_y x)" and
-          "buf_y x = CleanQ_RB_read_tail_valid_length_y (CRB x) (buf_y x)"
-  shows "CleanQ_RB_read_tail_flags_y (CRB x) (buf_y x) = CleanQ_RB_read_tail_y (CRB x)"
-  unfolding CleanQ_RB_read_tail_flags_y_def
-  by (metis CleanQ_Buffer.surjective CleanQ_Buffer.update_convs(4) CleanQ_Buffer.update_convs(5) 
-      CleanQ_Buffer.update_convs(6) CleanQ_RB_read_tail_flags_y_def CleanQ_RB_read_tail_valid_length_y_def 
-      CleanQ_RB_read_tail_valid_offset_y_def CleanQ_RB_read_tail_y_fields_eq assms(1) assms(2) assms(3) assms(4) assms(5))
+lemma CleanQ_RB_read_tail_x_offset:
+  "b = CleanQ_RB_read_tail_region_x rb (b) \<Longrightarrow> b = CleanQ_RB_read_tail_flags_x rb (b) 
+    \<Longrightarrow> b = CleanQ_RB_read_tail_length_x rb (b) 
+    \<Longrightarrow> b = CleanQ_RB_read_tail_valid_offset_x rb (b) 
+    \<Longrightarrow> b = CleanQ_RB_read_tail_valid_length_x rb (b) \<Longrightarrow> 
+      CleanQ_RB_read_tail_offset_x rb (b) = CleanQ_RB_read_tail_x rb"
+  by (metis CleanQ_RB_read_tail_flags_x_offset_x CleanQ_RB_read_tail_length_x_offset_x 
+            CleanQ_RB_read_tail_valid_length_x_offset_x CleanQ_RB_read_tail_valid_offset_x_offset_x 
+             CleanQ_RB_read_tail_x_fields_eq)
 
-lemma CleanQ_RB_read_tail_x_flags [simp]:
-  assumes "buf_x x = CleanQ_RB_read_tail_region_x (CRB x) (buf_x x)" and
-          "buf_x x = CleanQ_RB_read_tail_offset_x (CRB x) (buf_x x)" and
-          "buf_x x = CleanQ_RB_read_tail_length_x (CRB x) (buf_x x)" and
-          "buf_x x = CleanQ_RB_read_tail_valid_offset_x (CRB x) (buf_x x)" and
-          "buf_x x = CleanQ_RB_read_tail_valid_length_x (CRB x) (buf_x x)"
-  shows "CleanQ_RB_read_tail_flags_x (CRB x) (buf_x x) = CleanQ_RB_read_tail_x (CRB x)"
-  unfolding CleanQ_RB_read_tail_flags_x_def
-  by (metis CleanQ_Buffer.surjective CleanQ_Buffer.update_convs(4) CleanQ_Buffer.update_convs(5) 
-      CleanQ_Buffer.update_convs(6) CleanQ_RB_read_tail_flags_x_def CleanQ_RB_read_tail_valid_length_x_def 
-      CleanQ_RB_read_tail_valid_offset_x_def CleanQ_RB_read_tail_x_fields_eq assms(1) assms(2) assms(3) assms(4) assms(5)) 
+lemma CleanQ_RB_read_tail_x_length:
+  "b = CleanQ_RB_read_tail_region_x rb (b) \<Longrightarrow> b = CleanQ_RB_read_tail_offset_x rb (b) 
+    \<Longrightarrow> b = CleanQ_RB_read_tail_flags_x rb (b) 
+    \<Longrightarrow> b = CleanQ_RB_read_tail_valid_offset_x rb (b) 
+    \<Longrightarrow> b = CleanQ_RB_read_tail_valid_length_x rb (b) \<Longrightarrow> 
+      CleanQ_RB_read_tail_length_x rb (b) = CleanQ_RB_read_tail_x rb"
+  by (metis CleanQ_RB_read_tail_flags_x_length_x CleanQ_RB_read_tail_valid_length_x_length_x
+            CleanQ_RB_read_tail_valid_offset_x_length_x CleanQ_RB_read_tail_x_fields_eq)
 
+lemma CleanQ_RB_read_tail_x_valid_offset:
+  "b = CleanQ_RB_read_tail_region_x rb (b) \<Longrightarrow> b = CleanQ_RB_read_tail_offset_x rb (b) 
+    \<Longrightarrow> b = CleanQ_RB_read_tail_length_x rb (b) 
+    \<Longrightarrow> b = CleanQ_RB_read_tail_flags_x rb (b) 
+    \<Longrightarrow> b = CleanQ_RB_read_tail_valid_length_x rb (b) \<Longrightarrow> 
+      CleanQ_RB_read_tail_valid_offset_x rb (b) = CleanQ_RB_read_tail_x rb"
+  by (metis CleanQ_RB_read_tail_x_fields_eq)
 
+lemma CleanQ_RB_read_tail_x_valid_length:
+  "b = CleanQ_RB_read_tail_region_x rb (b) \<Longrightarrow> b = CleanQ_RB_read_tail_offset_x rb (b) 
+    \<Longrightarrow> b = CleanQ_RB_read_tail_length_x rb (b) 
+    \<Longrightarrow> b = CleanQ_RB_read_tail_valid_offset_x rb (b) 
+    \<Longrightarrow> b = CleanQ_RB_read_tail_flags_x rb (b) \<Longrightarrow> 
+      CleanQ_RB_read_tail_valid_length_x rb (b) = CleanQ_RB_read_tail_x rb"
+  by (metis CleanQ_RB_read_tail_valid_offset_x_valid_length_x CleanQ_RB_read_tail_x_fields_eq)
 
-(* ------------------------------------------------------------------------------------ *)
-subsubsection \<open>Defining enqueue and deuque for Complx\<close>
-(* ------------------------------------------------------------------------------------ *)
+lemma CleanQ_RB_read_tail_x_flags[simp]:
+  "b = CleanQ_RB_read_tail_region_x rb (b) \<Longrightarrow> b = CleanQ_RB_read_tail_offset_x rb (b) 
+    \<Longrightarrow> b = CleanQ_RB_read_tail_length_x rb (b) 
+    \<Longrightarrow> b = CleanQ_RB_read_tail_valid_offset_x rb (b) 
+    \<Longrightarrow> b = CleanQ_RB_read_tail_valid_length_x rb (b) \<Longrightarrow> 
+      CleanQ_RB_read_tail_flags_x rb (b) = CleanQ_RB_read_tail_x rb"
+  by (metis CleanQ_RB_read_tail_valid_length_x_flags_x CleanQ_RB_read_tail_valid_offset_x_flags_x 
+            CleanQ_RB_read_tail_x_fields_eq)
 
-
-abbreviation "CleanQ_CRB_enq_x b \<equiv> 
-            \<lbrace> CleanQ_RB_Invariants \<acute>uni \<acute>CRB  \<rbrace>
-            IF CleanQ_RB_enq_x_possible \<acute>CRB \<and> b \<in> rSX \<acute>CRB
-            THEN
-              \<lbrace> CleanQ_RB_enq_x_P \<acute>uni \<acute>CRB b \<rbrace>
-                \<acute>CRB := (CleanQ_RB_write_head_x b \<acute>CRB) ;;
-              \<lbrace> CleanQ_RB_enq_x_Q \<acute>uni \<acute>CRB b \<rbrace>
-                \<acute>CRB := (CleanQ_RB_incr_head_x b \<acute>CRB)
-            ELSE 
-                \<lbrace>  CleanQ_RB_Invariants \<acute>uni \<acute>CRB \<rbrace>
-                SKIP
-            FI"
-
-abbreviation "CleanQ_CRB_enq_y b \<equiv> 
-            \<lbrace> CleanQ_RB_Invariants \<acute>uni \<acute>CRB  \<rbrace>
-            IF CleanQ_RB_enq_y_possible \<acute>CRB \<and> b \<in> rSY \<acute>CRB
-            THEN
-              \<lbrace> CleanQ_RB_enq_y_P \<acute>uni \<acute>CRB b \<rbrace>
-                \<acute>CRB := (CleanQ_RB_write_head_y b \<acute>CRB) ;;
-              \<lbrace> CleanQ_RB_enq_y_Q \<acute>uni \<acute>CRB b \<rbrace>
-                \<acute>CRB := (CleanQ_RB_incr_head_y b \<acute>CRB)
-            ELSE 
-                \<lbrace>  CleanQ_RB_Invariants \<acute>uni \<acute>CRB \<rbrace>
-                SKIP
-            FI"
-
-abbreviation "CleanQ_CRB_deq_x \<equiv> 
-            \<lbrace> CleanQ_RB_Invariants \<acute>uni \<acute>CRB  \<rbrace>
-            IF CleanQ_RB_deq_x_possible \<acute>CRB
-            THEN
-              \<lbrace> CleanQ_RB_deq_x_P \<acute>uni \<acute>CRB (CleanQ_RB_read_tail_x \<acute>CRB) \<rbrace>
-                \<acute>buf_x := (CleanQ_RB_read_tail_x  \<acute>CRB) ;;
-              \<lbrace> CleanQ_RB_deq_x_Q \<acute>uni \<acute>CRB \<acute>buf_x \<rbrace>
-                \<acute>CRB := (CleanQ_RB_incr_tail_x \<acute>buf_x \<acute>CRB)
-            ELSE 
-                \<lbrace>  CleanQ_RB_Invariants \<acute>uni \<acute>CRB \<rbrace>
-                SKIP
-            FI"
+lemmas CleanQ_RB_read_tail_x_fields_simp = 
+  CleanQ_RB_read_tail_x_region
+  CleanQ_RB_read_tail_x_offset
+  CleanQ_RB_read_tail_x_length
+  CleanQ_RB_read_tail_x_valid_offset
+  CleanQ_RB_read_tail_x_valid_length
+  CleanQ_RB_read_tail_x_flags
 
 
-abbreviation "CleanQ_CRB_deq_y \<equiv> 
-            \<lbrace> CleanQ_RB_Invariants \<acute>uni \<acute>CRB  \<rbrace>
-            IF CleanQ_RB_deq_y_possible \<acute>CRB
-            THEN
-              \<lbrace> CleanQ_RB_deq_y_P \<acute>uni \<acute>CRB (CleanQ_RB_read_tail_y \<acute>CRB) \<rbrace>
-                \<acute>buf_y := (CleanQ_RB_read_tail_y  \<acute>CRB) ;;
-              \<lbrace> CleanQ_RB_deq_y_Q \<acute>uni \<acute>CRB \<acute>buf_y \<rbrace>
-                \<acute>CRB := (CleanQ_RB_incr_tail_y \<acute>buf_y \<acute>CRB)
-            ELSE 
-                \<lbrace>  CleanQ_RB_Invariants \<acute>uni \<acute>CRB \<rbrace>
-                SKIP
-            FI"
-
-abbreviation "CleanQ_CRB_enq_mult_x b \<equiv> 
-            \<lbrace> CleanQ_RB_Invariants \<acute>uni \<acute>CRB  \<rbrace>
-            IF CleanQ_RB_enq_x_possible \<acute>CRB \<and> b \<in> rSX \<acute>CRB
-            THEN
-              \<lbrace> CleanQ_RB_enq_x_P \<acute>uni \<acute>CRB b \<rbrace>
-                \<acute>CRB := (CleanQ_RB_write_head_region_x ( b) \<acute>CRB) ;;
-              \<lbrace> CleanQ_RB_enq_x_P \<acute>uni \<acute>CRB b \<and> 
-                region (CleanQ_RB_read_head_x \<acute>CRB) = region b 
-              \<rbrace>
-                \<acute>CRB := (CleanQ_RB_write_head_offset_x ( b) \<acute>CRB) ;;
-              \<lbrace> CleanQ_RB_enq_x_P \<acute>uni \<acute>CRB b \<and> 
-                region (CleanQ_RB_read_head_x \<acute>CRB) = region b \<and>
-                offset (CleanQ_RB_read_head_x \<acute>CRB) = offset b 
-              \<rbrace>
-                \<acute>CRB := (CleanQ_RB_write_head_length_x ( b) \<acute>CRB) ;;
-              \<lbrace> CleanQ_RB_enq_x_P \<acute>uni \<acute>CRB b \<and> 
-                region (CleanQ_RB_read_head_x \<acute>CRB) = region b \<and>
-                offset (CleanQ_RB_read_head_x \<acute>CRB) = offset b \<and>
-                length (CleanQ_RB_read_head_x \<acute>CRB) = length b
-              \<rbrace>
-                \<acute>CRB := (CleanQ_RB_write_head_valid_offset_x ( b) \<acute>CRB) ;;
-              \<lbrace> CleanQ_RB_enq_x_P \<acute>uni \<acute>CRB b \<and> 
-                region (CleanQ_RB_read_head_x \<acute>CRB) = region b \<and>
-                offset (CleanQ_RB_read_head_x \<acute>CRB) = offset b \<and>
-                length (CleanQ_RB_read_head_x \<acute>CRB) = length b \<and>
-                valid_offset (CleanQ_RB_read_head_x \<acute>CRB) = valid_offset b
-              \<rbrace>
-                \<acute>CRB := (CleanQ_RB_write_head_valid_length_x ( b) \<acute>CRB) ;;
-              \<lbrace> CleanQ_RB_enq_x_P \<acute>uni \<acute>CRB b \<and> 
-                region (CleanQ_RB_read_head_x \<acute>CRB) = region b \<and>
-                offset (CleanQ_RB_read_head_x \<acute>CRB) = offset b \<and>
-                length (CleanQ_RB_read_head_x \<acute>CRB) = length b \<and>
-                valid_offset (CleanQ_RB_read_head_x \<acute>CRB) = valid_offset b \<and>
-                valid_length (CleanQ_RB_read_head_x \<acute>CRB) = valid_length b
-              \<rbrace>
-                \<acute>CRB := (CleanQ_RB_write_head_flags_x ( b) \<acute>CRB) ;;
-              \<lbrace> CleanQ_RB_enq_x_Q \<acute>uni \<acute>CRB b \<rbrace>
-                \<acute>CRB := (CleanQ_RB_incr_head_x b \<acute>CRB)
-            ELSE 
-                \<lbrace>  CleanQ_RB_Invariants \<acute>uni \<acute>CRB \<rbrace>
-                SKIP
-            FI"
-
-abbreviation "CleanQ_CRB_enq_mult_y b \<equiv> 
-            \<lbrace> CleanQ_RB_Invariants \<acute>uni \<acute>CRB  \<rbrace>
-            IF CleanQ_RB_enq_y_possible \<acute>CRB \<and> b \<in> rSY \<acute>CRB
-            THEN
-              \<lbrace> CleanQ_RB_enq_y_P \<acute>uni \<acute>CRB b \<rbrace>
-                \<acute>CRB := (CleanQ_RB_write_head_region_y ( b) \<acute>CRB) ;;
-              \<lbrace> CleanQ_RB_enq_y_P \<acute>uni \<acute>CRB b \<and> 
-                region (CleanQ_RB_read_head_y \<acute>CRB) = region b 
-              \<rbrace>
-                \<acute>CRB := (CleanQ_RB_write_head_offset_y ( b) \<acute>CRB) ;;
-              \<lbrace> CleanQ_RB_enq_y_P \<acute>uni \<acute>CRB b \<and>  
-                region (CleanQ_RB_read_head_y \<acute>CRB) = region b \<and>
-                offset (CleanQ_RB_read_head_y \<acute>CRB) = offset b 
-              \<rbrace>
-                \<acute>CRB := (CleanQ_RB_write_head_length_y ( b) \<acute>CRB) ;;
-              \<lbrace> CleanQ_RB_enq_y_P \<acute>uni \<acute>CRB b \<and>  
-                region (CleanQ_RB_read_head_y \<acute>CRB) = region b \<and>
-                offset (CleanQ_RB_read_head_y \<acute>CRB) = offset b \<and>
-                length (CleanQ_RB_read_head_y \<acute>CRB) = length b 
-              \<rbrace>
-                \<acute>CRB := (CleanQ_RB_write_head_valid_offset_y ( b) \<acute>CRB) ;;
-              \<lbrace> CleanQ_RB_enq_y_P \<acute>uni \<acute>CRB b \<and>  
-                region (CleanQ_RB_read_head_y \<acute>CRB) = region b \<and>
-                offset (CleanQ_RB_read_head_y \<acute>CRB) = offset b \<and>
-                length (CleanQ_RB_read_head_y \<acute>CRB) = length b \<and> 
-                valid_offset (CleanQ_RB_read_head_y \<acute>CRB) = valid_offset b
-              \<rbrace>
-                \<acute>CRB := (CleanQ_RB_write_head_valid_length_y ( b) \<acute>CRB) ;;
-              \<lbrace> CleanQ_RB_enq_y_P \<acute>uni \<acute>CRB b \<and>  
-                region (CleanQ_RB_read_head_y \<acute>CRB) = region b \<and>
-                offset (CleanQ_RB_read_head_y \<acute>CRB) = offset b \<and>
-                length (CleanQ_RB_read_head_y \<acute>CRB) = length b \<and> 
-                valid_offset (CleanQ_RB_read_head_y \<acute>CRB) = valid_offset b \<and>
-                valid_length (CleanQ_RB_read_head_y \<acute>CRB) = valid_length b
-              \<rbrace>
-                \<acute>CRB := (CleanQ_RB_write_head_flags_y ( b) \<acute>CRB) ;;
-              \<lbrace> CleanQ_RB_enq_y_Q \<acute>uni \<acute>CRB b \<rbrace>
-                \<acute>CRB := (CleanQ_RB_incr_head_y b \<acute>CRB)
-            ELSE 
-                \<lbrace>  CleanQ_RB_Invariants \<acute>uni \<acute>CRB \<rbrace>
-                SKIP
-            FI"
-
-abbreviation "CleanQ_CRB_deq_mult_x \<equiv> 
-            \<lbrace> CleanQ_RB_Invariants \<acute>uni \<acute>CRB  \<rbrace>
-            IF CleanQ_RB_deq_x_possible \<acute>CRB
-            THEN
-              \<lbrace> CleanQ_RB_deq_x_P \<acute>uni \<acute>CRB (CleanQ_RB_read_tail_x \<acute>CRB) \<rbrace>
-                \<acute>buf_x := (CleanQ_RB_read_tail_region_x \<acute>CRB \<acute>buf_x) ;;
-              \<lbrace> CleanQ_RB_deq_x_P \<acute>uni \<acute>CRB (CleanQ_RB_read_tail_x \<acute>CRB) \<and>
-                \<acute>buf_x = CleanQ_RB_read_tail_region_x \<acute>CRB \<acute>buf_x
-              \<rbrace>
-                \<acute>buf_x := (CleanQ_RB_read_tail_offset_x \<acute>CRB \<acute>buf_x) ;;
-              \<lbrace> CleanQ_RB_deq_x_P \<acute>uni \<acute>CRB (CleanQ_RB_read_tail_x \<acute>CRB) \<and>
-                \<acute>buf_x = CleanQ_RB_read_tail_region_x \<acute>CRB \<acute>buf_x \<and>
-                \<acute>buf_x = CleanQ_RB_read_tail_offset_x \<acute>CRB \<acute>buf_x
-              \<rbrace>
-                \<acute>buf_x := (CleanQ_RB_read_tail_length_x \<acute>CRB \<acute>buf_x) ;;
-              \<lbrace> CleanQ_RB_deq_x_P \<acute>uni \<acute>CRB (CleanQ_RB_read_tail_x \<acute>CRB) \<and>
-                \<acute>buf_x = CleanQ_RB_read_tail_region_x \<acute>CRB \<acute>buf_x \<and>
-                \<acute>buf_x = CleanQ_RB_read_tail_offset_x \<acute>CRB \<acute>buf_x \<and>
-                \<acute>buf_x = CleanQ_RB_read_tail_length_x \<acute>CRB \<acute>buf_x 
-              \<rbrace>
-                \<acute>buf_x := (CleanQ_RB_read_tail_valid_offset_x \<acute>CRB \<acute>buf_x) ;;
-              \<lbrace> CleanQ_RB_deq_x_P \<acute>uni \<acute>CRB (CleanQ_RB_read_tail_x \<acute>CRB) \<and>
-                \<acute>buf_x = CleanQ_RB_read_tail_region_x \<acute>CRB \<acute>buf_x \<and>
-                \<acute>buf_x = CleanQ_RB_read_tail_offset_x \<acute>CRB \<acute>buf_x \<and>
-                \<acute>buf_x = CleanQ_RB_read_tail_length_x \<acute>CRB \<acute>buf_x \<and>
-                \<acute>buf_x = CleanQ_RB_read_tail_valid_offset_x \<acute>CRB \<acute>buf_x 
-              \<rbrace>
-                \<acute>buf_x := (CleanQ_RB_read_tail_valid_length_x \<acute>CRB \<acute>buf_x) ;;
-              \<lbrace> CleanQ_RB_deq_x_P \<acute>uni \<acute>CRB (CleanQ_RB_read_tail_x \<acute>CRB) \<and>
-                \<acute>buf_x = CleanQ_RB_read_tail_region_x \<acute>CRB \<acute>buf_x \<and>
-                \<acute>buf_x = CleanQ_RB_read_tail_offset_x \<acute>CRB \<acute>buf_x \<and>
-                \<acute>buf_x = CleanQ_RB_read_tail_length_x \<acute>CRB \<acute>buf_x \<and>
-                \<acute>buf_x = CleanQ_RB_read_tail_valid_offset_x \<acute>CRB \<acute>buf_x \<and>
-                \<acute>buf_x = CleanQ_RB_read_tail_valid_length_x \<acute>CRB \<acute>buf_x 
-              \<rbrace>
-                \<acute>buf_x := (CleanQ_RB_read_tail_flags_x \<acute>CRB \<acute>buf_x) ;;
-              \<lbrace> CleanQ_RB_deq_x_Q \<acute>uni \<acute>CRB \<acute>buf_x\<rbrace>
-                \<acute>CRB := (CleanQ_RB_incr_tail_x \<acute>buf_x \<acute>CRB)
-            ELSE 
-                \<lbrace>  CleanQ_RB_Invariants \<acute>uni \<acute>CRB \<rbrace>
-                SKIP
-            FI"
-
-abbreviation "CleanQ_CRB_deq_mult_y \<equiv> 
-            \<lbrace> CleanQ_RB_Invariants \<acute>uni \<acute>CRB  \<rbrace>
-            IF CleanQ_RB_deq_y_possible \<acute>CRB
-            THEN
-              \<lbrace> CleanQ_RB_deq_y_P \<acute>uni \<acute>CRB (CleanQ_RB_read_tail_y \<acute>CRB) \<rbrace>
-                \<acute>buf_y := (CleanQ_RB_read_tail_region_y \<acute>CRB \<acute>buf_y) ;;
-              \<lbrace> CleanQ_RB_deq_y_P \<acute>uni \<acute>CRB (CleanQ_RB_read_tail_y \<acute>CRB) \<and>
-                \<acute>buf_y = CleanQ_RB_read_tail_region_y \<acute>CRB \<acute>buf_y
-              \<rbrace>
-                \<acute>buf_y := (CleanQ_RB_read_tail_offset_y \<acute>CRB \<acute>buf_y) ;;
-              \<lbrace> CleanQ_RB_deq_y_P \<acute>uni \<acute>CRB (CleanQ_RB_read_tail_y \<acute>CRB) \<and>
-                \<acute>buf_y = CleanQ_RB_read_tail_region_y \<acute>CRB \<acute>buf_y \<and>
-                \<acute>buf_y = CleanQ_RB_read_tail_offset_y \<acute>CRB \<acute>buf_y
-              \<rbrace>
-                \<acute>buf_y := (CleanQ_RB_read_tail_length_y \<acute>CRB \<acute>buf_y) ;;
-              \<lbrace> CleanQ_RB_deq_y_P \<acute>uni \<acute>CRB (CleanQ_RB_read_tail_y \<acute>CRB) \<and>
-                \<acute>buf_y = CleanQ_RB_read_tail_region_y \<acute>CRB \<acute>buf_y \<and>
-                \<acute>buf_y = CleanQ_RB_read_tail_offset_y \<acute>CRB \<acute>buf_y \<and>
-                \<acute>buf_y = CleanQ_RB_read_tail_length_y \<acute>CRB \<acute>buf_y
-              \<rbrace>
-                \<acute>buf_y := (CleanQ_RB_read_tail_valid_offset_y \<acute>CRB \<acute>buf_y) ;;
-              \<lbrace> CleanQ_RB_deq_y_P \<acute>uni \<acute>CRB (CleanQ_RB_read_tail_y \<acute>CRB) \<and>
-                \<acute>buf_y = CleanQ_RB_read_tail_region_y \<acute>CRB \<acute>buf_y \<and>
-                \<acute>buf_y = CleanQ_RB_read_tail_offset_y \<acute>CRB \<acute>buf_y \<and>
-                \<acute>buf_y = CleanQ_RB_read_tail_length_y \<acute>CRB \<acute>buf_y \<and>
-                \<acute>buf_y = CleanQ_RB_read_tail_valid_offset_y \<acute>CRB \<acute>buf_y
-              \<rbrace>
-                \<acute>buf_y := (CleanQ_RB_read_tail_valid_length_y \<acute>CRB \<acute>buf_y) ;;
-              \<lbrace> CleanQ_RB_deq_y_P \<acute>uni \<acute>CRB (CleanQ_RB_read_tail_y \<acute>CRB) \<and>
-                \<acute>buf_y = CleanQ_RB_read_tail_region_y \<acute>CRB \<acute>buf_y \<and>
-                \<acute>buf_y = CleanQ_RB_read_tail_offset_y \<acute>CRB \<acute>buf_y \<and>
-                \<acute>buf_y = CleanQ_RB_read_tail_length_y \<acute>CRB \<acute>buf_y \<and>
-                \<acute>buf_y = CleanQ_RB_read_tail_valid_offset_y \<acute>CRB \<acute>buf_y \<and>
-                \<acute>buf_y = CleanQ_RB_read_tail_valid_length_y \<acute>CRB \<acute>buf_y
-              \<rbrace>
-                \<acute>buf_y := (CleanQ_RB_read_tail_flags_y \<acute>CRB \<acute>buf_y) ;;
-              \<lbrace> CleanQ_RB_deq_y_Q \<acute>uni \<acute>CRB \<acute>buf_y \<rbrace>
-                \<acute>CRB := (CleanQ_RB_incr_tail_y \<acute>buf_y \<acute>CRB)
-            ELSE 
-                \<lbrace>  CleanQ_RB_Invariants \<acute>uni \<acute>CRB \<rbrace>
-                SKIP
-            FI"
-(* ------------------------------------------------------------------------------------ *)
-subsubsection \<open>Hoare Triples for the Enqueue Operation\<close>
-(* ------------------------------------------------------------------------------------ *)
+(* ==================================================================================== *)
+subsection \<open>Hoare Triples for the Enqueue Operation\<close>
+(* ==================================================================================== *)
 
 
 text \<open>
   We now show that the \verb+enqueue+ operation satisfies the pre and post conditions
-  for the predicates P, Q and R. 
+  for the predicates P, Q and R. Note this does not include parallel structures yet.
+  We do this to show the equivalence to the sequential part. We first show this for
+  the two elements and then for the entire operation.
 \<close>
-
 
 paragraph \<open>Writing the Head Element\<close>
 
@@ -4147,20 +4106,17 @@ text \<open>
 
 lemma  CleanQ_RB_write_head_x_hoare:
   "\<Gamma>, \<Theta> |\<turnstile>\<^bsub>/ F\<^esub> 
-   \<lbrace> CleanQ_RB_enq_x_P K \<acute>CRB b \<rbrace> 
+  \<lbrace> CleanQ_RB_enq_x_P K \<acute>CRB b \<rbrace> 
     \<acute>CRB := (CleanQ_RB_write_head_x b \<acute>CRB)
-   \<lbrace> CleanQ_RB_enq_x_Q K \<acute>CRB b  \<rbrace>, \<lbrace>True\<rbrace>"     
-  apply(oghoare)
-  by simp
-  
+  \<lbrace> CleanQ_RB_enq_x_Q K \<acute>CRB b  \<rbrace>, \<lbrace>True\<rbrace>"     
+  by(oghoare, auto)  
 
 lemma  CleanQ_RB_write_head_y_hoare:
- "\<Gamma>, \<Theta> |\<turnstile>\<^bsub>/ F\<^esub> 
-      \<lbrace> CleanQ_RB_enq_y_P K \<acute>CRB b \<rbrace> 
-        \<acute>CRB := (CleanQ_RB_write_head_y b \<acute>CRB)
-      \<lbrace> CleanQ_RB_enq_y_Q K \<acute> CRB b  \<rbrace>, \<lbrace>True\<rbrace>"                                                 
-  apply(oghoare)
-  by simp
+  "\<Gamma>, \<Theta> |\<turnstile>\<^bsub>/ F\<^esub> 
+  \<lbrace> CleanQ_RB_enq_y_P K \<acute>CRB b \<rbrace> 
+    \<acute>CRB := (CleanQ_RB_write_head_y b \<acute>CRB)
+  \<lbrace> CleanQ_RB_enq_y_Q K \<acute> CRB b  \<rbrace>, \<lbrace>True\<rbrace>"                                                 
+  by(oghoare, auto)
 
 
 paragraph \<open>Incrementing the Head Pointer\<close>
@@ -4170,40 +4126,35 @@ text \<open>
 \<close>
 
 lemma  CleanQ_RB_incr_head_x_hoare:
-   "\<Gamma>, \<Theta> |\<turnstile>\<^bsub>/ F\<^esub> 
-    \<lbrace> CleanQ_RB_enq_x_Q K \<acute>CRB b \<rbrace> 
-        \<acute>CRB := (CleanQ_RB_incr_head_x b \<acute>CRB)
-    \<lbrace> CleanQ_RB_enq_x_R K \<acute>CRB b  \<rbrace>, \<lbrace>True\<rbrace>"
-  apply(oghoare)
-  using CleanQ_RB_enq_x_inv_all CleanQ_RB_enq_x_result by fastforce
+  "\<Gamma>, \<Theta> |\<turnstile>\<^bsub>/ F\<^esub> 
+  \<lbrace> CleanQ_RB_enq_x_Q K \<acute>CRB b \<rbrace> 
+    \<acute>CRB := (CleanQ_RB_incr_head_x b \<acute>CRB)
+  \<lbrace> CleanQ_RB_enq_x_R K \<acute>CRB b  \<rbrace>, \<lbrace>True\<rbrace>"
+  by(oghoare, auto)
 
 lemma  CleanQ_RB_incr_head_y_hoare:
   "\<Gamma>, \<Theta> |\<turnstile>\<^bsub>/ F\<^esub>  
-    \<lbrace>  CleanQ_RB_enq_y_Q K \<acute>CRB b \<rbrace> 
-        \<acute>CRB := (CleanQ_RB_incr_head_y b \<acute>CRB)
-    \<lbrace> CleanQ_RB_enq_y_R K \<acute>CRB b  \<rbrace>, \<lbrace>True\<rbrace>"
-  apply(oghoare)
-  using CleanQ_RB_enq_y_inv_all CleanQ_RB_enq_y_result by fastforce
+  \<lbrace> CleanQ_RB_enq_y_Q K \<acute>CRB b \<rbrace> 
+    \<acute>CRB := (CleanQ_RB_incr_head_y b \<acute>CRB)
+  \<lbrace> CleanQ_RB_enq_y_R K \<acute>CRB b  \<rbrace>, \<lbrace>True\<rbrace>"
+  by(oghoare, auto) 
 
 
 paragraph \<open>Full Enqueue Operation\<close>
 
 text \<open>
-  We show the Hoare triple with \verb+{P) enq {R}+.
+  We show the full Hoare triple with \verb+{P) enq {R}+.
 \<close>
 
 lemma CleanQ_RB_enq_x_hoare : 
   "\<Gamma>, \<Theta> |\<turnstile>\<^bsub>/ F\<^esub>  
-   \<lbrace> CleanQ_RB_enq_x_P K \<acute>CRB b \<rbrace> 
+  \<lbrace> CleanQ_RB_enq_x_P K \<acute>CRB b \<rbrace> 
     \<acute>CRB := (CleanQ_RB_write_head_x b \<acute>CRB) ;;
-   \<lbrace> CleanQ_RB_enq_x_Q K \<acute>CRB b \<rbrace>
-     \<acute>CRB := (CleanQ_RB_incr_head_x b \<acute>CRB)
-   \<lbrace> CleanQ_RB_enq_x_R K \<acute>CRB b \<rbrace>, \<lbrace>True\<rbrace>"
-  apply(oghoare)
-  using CleanQ_RB_enq_x_inv_all CleanQ_RB_enq_x_result apply fastforce
-  by simp
-  
-
+  \<lbrace> CleanQ_RB_enq_x_Q K \<acute>CRB b \<rbrace>
+    \<acute>CRB := (CleanQ_RB_incr_head_x b \<acute>CRB)
+  \<lbrace> CleanQ_RB_enq_x_R K \<acute>CRB b \<rbrace>, \<lbrace>True\<rbrace>"
+  by(oghoare, auto)
+ 
 lemma CleanQ_RB_enq_y_hoare : 
   "\<Gamma>, \<Theta> |\<turnstile>\<^bsub>/ F\<^esub>  
   \<lbrace> CleanQ_RB_enq_y_P K \<acute>CRB b \<rbrace> 
@@ -4211,14 +4162,191 @@ lemma CleanQ_RB_enq_y_hoare :
   \<lbrace> CleanQ_RB_enq_y_Q K \<acute>CRB b \<rbrace>
     \<acute>CRB := (CleanQ_RB_incr_head_y b \<acute>CRB)
   \<lbrace> CleanQ_RB_enq_y_R K \<acute>CRB b \<rbrace>, \<lbrace>True\<rbrace>"
-  apply(oghoare)
-  using CleanQ_RB_enq_y_inv_all CleanQ_RB_enq_y_result apply fastforce
-  by simp
+  by(oghoare, auto)
 
 
-(* ------------------------------------------------------------------------------------ *)
-subsubsection \<open>Hoare Triples for the Dequeue Operation\<close>
-(* ------------------------------------------------------------------------------------ *)
+text \<open>
+  Last we show that the enqueue in two steps is the same as the big step enqueue.
+\<close>
+
+lemma CleanQ_RB_enq_x_hoare_enq_equiv : 
+  "\<Gamma>, \<Theta> |\<turnstile>\<^bsub>/ F\<^esub>  
+  \<lbrace> CleanQ_RB_enq_x_P K \<acute>CRB b \<and> \<acute>CRB = rb \<rbrace> 
+    \<acute>CRB := (CleanQ_RB_write_head_x b \<acute>CRB) ;;
+  \<lbrace> CleanQ_RB_enq_x_Q K \<acute>CRB b \<and> \<acute>CRB = CleanQ_RB_write_head_x b rb \<rbrace>
+    \<acute>CRB := (CleanQ_RB_incr_head_x b \<acute>CRB)
+  \<lbrace> CleanQ_RB_enq_x_R K \<acute>CRB b \<and> \<acute>CRB = CleanQ_RB_enq_x b rb \<rbrace>, \<lbrace>True\<rbrace>"
+  apply(oghoare, auto)
+  by (metis CleanQ_RB_enq_x_equiv_incr_head CleanQ_RB_enq_x_split_equal)
+
+lemma CleanQ_RB_enq_y_hoare_enq_equiv : 
+  "\<Gamma>, \<Theta> |\<turnstile>\<^bsub>/ F\<^esub>  
+  \<lbrace> CleanQ_RB_enq_y_P K \<acute>CRB b \<and> \<acute>CRB = rb \<rbrace> 
+    \<acute>CRB := (CleanQ_RB_write_head_y b \<acute>CRB) ;;
+  \<lbrace> CleanQ_RB_enq_y_Q K \<acute>CRB b \<and> \<acute>CRB = CleanQ_RB_write_head_y b rb \<rbrace>
+    \<acute>CRB := (CleanQ_RB_incr_head_y b \<acute>CRB)
+  \<lbrace> CleanQ_RB_enq_y_R K \<acute>CRB b \<and> \<acute>CRB = CleanQ_RB_enq_y b rb \<rbrace>, \<lbrace>True\<rbrace>"
+  apply(oghoare, auto)
+  by (metis CleanQ_RB_enq_y_equiv_incr_head CleanQ_RB_enq_y_split_equal)
+
+
+paragraph \<open>Conditional Enqueue\<close>
+
+text \<open>
+  We now define the \verb+Enqueue+ operation as a convenient abbreviation, which 
+  includes the a conditional that checks if we can enqueue something. 
+\<close>
+
+abbreviation "CleanQ_CRB_enq_x b \<equiv> 
+  \<lbrace> CleanQ_RB_Invariants \<acute>uni \<acute>CRB  \<rbrace>
+    IF CleanQ_RB_enq_x_possible \<acute>CRB \<and> b \<in> rSX \<acute>CRB
+    THEN
+      \<lbrace> CleanQ_RB_enq_x_P \<acute>uni \<acute>CRB b \<rbrace>
+        \<acute>CRB := (CleanQ_RB_write_head_x b \<acute>CRB) ;;
+      \<lbrace> CleanQ_RB_enq_x_Q \<acute>uni \<acute>CRB b \<rbrace>
+        \<acute>CRB := (CleanQ_RB_incr_head_x b \<acute>CRB) ;;
+      \<lbrace> CleanQ_RB_enq_x_R \<acute>uni \<acute>CRB b \<rbrace> 
+        SKIP
+    ELSE 
+      \<lbrace>  CleanQ_RB_Invariants \<acute>uni \<acute>CRB \<rbrace>
+        SKIP
+    FI"
+
+abbreviation "CleanQ_CRB_enq_y b \<equiv> 
+  \<lbrace> CleanQ_RB_Invariants \<acute>uni \<acute>CRB  \<rbrace>
+    IF CleanQ_RB_enq_y_possible \<acute>CRB \<and> b \<in> rSY \<acute>CRB
+    THEN
+      \<lbrace> CleanQ_RB_enq_y_P \<acute>uni \<acute>CRB b \<rbrace>
+        \<acute>CRB := (CleanQ_RB_write_head_y b \<acute>CRB) ;;
+      \<lbrace> CleanQ_RB_enq_y_Q \<acute>uni \<acute>CRB b \<rbrace>
+        \<acute>CRB := (CleanQ_RB_incr_head_y b \<acute>CRB) ;;
+      \<lbrace> CleanQ_RB_enq_y_R \<acute>uni \<acute>CRB b \<rbrace> 
+        SKIP
+    ELSE 
+      \<lbrace> CleanQ_RB_Invariants \<acute>uni \<acute>CRB \<rbrace>
+        SKIP
+    FI"
+
+paragraph \<open>Multistep Enqueue Operation\<close>
+
+text \<open>
+  Writing the entire record is not an atomic operation. So we define this as a sequence
+  of writing single fields in the record. 
+\<close>
+
+abbreviation "CleanQ_CRB_enq_mult_x b \<equiv> 
+  \<lbrace> CleanQ_RB_Invariants \<acute>uni \<acute>CRB  \<rbrace>
+    IF CleanQ_RB_enq_x_possible \<acute>CRB \<and> b \<in> rSX \<acute>CRB
+    THEN
+      \<lbrace> CleanQ_RB_enq_x_P \<acute>uni \<acute>CRB b \<rbrace>
+        \<acute>CRB := (CleanQ_RB_write_head_region_x ( b) \<acute>CRB) ;;
+      \<lbrace> CleanQ_RB_enq_x_P \<acute>uni \<acute>CRB b \<and> 
+        region (CleanQ_RB_read_head_x \<acute>CRB) = region b 
+      \<rbrace>
+        \<acute>CRB := (CleanQ_RB_write_head_offset_x ( b) \<acute>CRB) ;;
+      \<lbrace> CleanQ_RB_enq_x_P \<acute>uni \<acute>CRB b \<and> 
+        region (CleanQ_RB_read_head_x \<acute>CRB) = region b \<and>
+        offset (CleanQ_RB_read_head_x \<acute>CRB) = offset b 
+      \<rbrace>
+        \<acute>CRB := (CleanQ_RB_write_head_length_x ( b) \<acute>CRB) ;;
+      \<lbrace> CleanQ_RB_enq_x_P \<acute>uni \<acute>CRB b \<and> 
+        region (CleanQ_RB_read_head_x \<acute>CRB) = region b \<and>
+        offset (CleanQ_RB_read_head_x \<acute>CRB) = offset b \<and>
+        length (CleanQ_RB_read_head_x \<acute>CRB) = length b
+      \<rbrace>
+        \<acute>CRB := (CleanQ_RB_write_head_valid_offset_x ( b) \<acute>CRB) ;;
+      \<lbrace> CleanQ_RB_enq_x_P \<acute>uni \<acute>CRB b \<and> 
+        region (CleanQ_RB_read_head_x \<acute>CRB) = region b \<and>
+        offset (CleanQ_RB_read_head_x \<acute>CRB) = offset b \<and>
+        length (CleanQ_RB_read_head_x \<acute>CRB) = length b \<and>
+        valid_offset (CleanQ_RB_read_head_x \<acute>CRB) = valid_offset b
+      \<rbrace>
+        \<acute>CRB := (CleanQ_RB_write_head_valid_length_x ( b) \<acute>CRB) ;;
+      \<lbrace> CleanQ_RB_enq_x_P \<acute>uni \<acute>CRB b \<and> 
+        region (CleanQ_RB_read_head_x \<acute>CRB) = region b \<and>
+        offset (CleanQ_RB_read_head_x \<acute>CRB) = offset b \<and>
+        length (CleanQ_RB_read_head_x \<acute>CRB) = length b \<and>
+        valid_offset (CleanQ_RB_read_head_x \<acute>CRB) = valid_offset b \<and>
+        valid_length (CleanQ_RB_read_head_x \<acute>CRB) = valid_length b
+      \<rbrace>
+        \<acute>CRB := (CleanQ_RB_write_head_flags_x b \<acute>CRB) ;;
+      \<lbrace> CleanQ_RB_enq_x_Q \<acute>uni \<acute>CRB b \<rbrace>
+        \<acute>CRB := (CleanQ_RB_incr_head_x b \<acute>CRB);;
+      \<lbrace> CleanQ_RB_enq_x_R \<acute>uni \<acute>CRB b \<rbrace> 
+        SKIP
+    ELSE 
+      \<lbrace> CleanQ_RB_Invariants \<acute>uni \<acute>CRB \<rbrace>
+      SKIP
+    FI"
+
+abbreviation "CleanQ_CRB_enq_mult_y b \<equiv> 
+  \<lbrace> CleanQ_RB_Invariants \<acute>uni \<acute>CRB  \<rbrace>
+    IF CleanQ_RB_enq_y_possible \<acute>CRB \<and> b \<in> rSY \<acute>CRB
+    THEN
+      \<lbrace> CleanQ_RB_enq_y_P \<acute>uni \<acute>CRB b \<rbrace>
+        \<acute>CRB := (CleanQ_RB_write_head_region_y ( b) \<acute>CRB) ;;
+      \<lbrace> CleanQ_RB_enq_y_P \<acute>uni \<acute>CRB b \<and> 
+        region (CleanQ_RB_read_head_y \<acute>CRB) = region b 
+      \<rbrace>
+        \<acute>CRB := (CleanQ_RB_write_head_offset_y ( b) \<acute>CRB) ;;
+      \<lbrace> CleanQ_RB_enq_y_P \<acute>uni \<acute>CRB b \<and> 
+        region (CleanQ_RB_read_head_y \<acute>CRB) = region b \<and>
+        offset (CleanQ_RB_read_head_y \<acute>CRB) = offset b 
+      \<rbrace>
+        \<acute>CRB := (CleanQ_RB_write_head_length_y ( b) \<acute>CRB) ;;
+      \<lbrace> CleanQ_RB_enq_y_P \<acute>uni \<acute>CRB b \<and> 
+        region (CleanQ_RB_read_head_y \<acute>CRB) = region b \<and>
+        offset (CleanQ_RB_read_head_y \<acute>CRB) = offset b \<and>
+        length (CleanQ_RB_read_head_y \<acute>CRB) = length b
+      \<rbrace>
+        \<acute>CRB := (CleanQ_RB_write_head_valid_offset_y ( b) \<acute>CRB) ;;
+      \<lbrace> CleanQ_RB_enq_y_P \<acute>uni \<acute>CRB b \<and> 
+        region (CleanQ_RB_read_head_y \<acute>CRB) = region b \<and>
+        offset (CleanQ_RB_read_head_y \<acute>CRB) = offset b \<and>
+        length (CleanQ_RB_read_head_y \<acute>CRB) = length b \<and>
+        valid_offset (CleanQ_RB_read_head_y \<acute>CRB) = valid_offset b
+      \<rbrace>
+        \<acute>CRB := (CleanQ_RB_write_head_valid_length_y ( b) \<acute>CRB) ;;
+      \<lbrace> CleanQ_RB_enq_y_P \<acute>uni \<acute>CRB b \<and> 
+        region (CleanQ_RB_read_head_y \<acute>CRB) = region b \<and>
+        offset (CleanQ_RB_read_head_y \<acute>CRB) = offset b \<and>
+        length (CleanQ_RB_read_head_y \<acute>CRB) = length b \<and>
+        valid_offset (CleanQ_RB_read_head_y \<acute>CRB) = valid_offset b \<and>
+        valid_length (CleanQ_RB_read_head_y \<acute>CRB) = valid_length b
+      \<rbrace>
+        \<acute>CRB := (CleanQ_RB_write_head_flags_y b \<acute>CRB) ;;
+      \<lbrace> CleanQ_RB_enq_y_Q \<acute>uni \<acute>CRB b \<rbrace>
+        \<acute>CRB := (CleanQ_RB_incr_head_y b \<acute>CRB);;
+      \<lbrace> CleanQ_RB_enq_y_R \<acute>uni \<acute>CRB b \<rbrace> 
+        SKIP
+    ELSE 
+      \<lbrace> CleanQ_RB_Invariants \<acute>uni \<acute>CRB \<rbrace>
+      SKIP
+    FI"
+
+
+paragraph \<open>Also do the conditional multistep?\<close>
+
+definition CleanQ_RB_transfer_buf_rsy :: "'a \<Rightarrow> 'a CleanQ_RB_State \<Rightarrow> 'a CleanQ_RB_State" 
+  where "CleanQ_RB_transfer_buf_rsy b rb = rb \<lparr>rSY := (rSY rb) - {b} \<rparr>"
+
+lemma CleanQ_RB_incr_head_y_mult : 
+  "\<Gamma>, \<Theta> |\<turnstile>\<^bsub>/ F\<^esub>  
+  \<lbrace>  CleanQ_RB_enq_y_Q \<acute>uni \<acute>CRB b \<and> rb =\<acute>CRB \<rbrace> 
+    \<acute>head_y := CleanQ_RB_read_head_tx_y \<acute>CRB ;;
+  \<lbrace> \<acute>head_y = CleanQ_RB_read_head_tx_y \<acute>CRB \<and> rb =\<acute>CRB \<rbrace>
+    \<acute>size_y := CleanQ_RB_read_size_tx_y \<acute>CRB ;;
+  \<lbrace> \<acute>head_y = CleanQ_RB_read_head_tx_y \<acute>CRB \<and> \<acute>size_y = CleanQ_RB_read_size_tx_y \<acute>CRB \<and> rb =\<acute>CRB  \<rbrace>
+    \<acute>CRB := (CleanQ_RB_write_headptr_y ((\<acute>head_y + 1) mod \<acute>size_y) (CleanQ_RB_transfer_buf_rsy b rb))
+  \<lbrace>  CleanQ_RB_enq_y_R \<acute>uni \<acute>CRB b \<and> \<acute>CRB = CleanQ_RB_incr_head_y b rb \<rbrace> , \<lbrace>True\<rbrace>"
+  apply(oghoare, auto)
+  oops
+  
+
+
+(* ==================================================================================== *)
+subsection \<open>Hoare Triples for the Dequeue Operation\<close>
+(* ==================================================================================== *)
 
 
 text \<open>
@@ -4248,6 +4376,7 @@ lemma  CleanQ_RB_read_tail_y_hoare:
   \<lbrace> CleanQ_RB_deq_y_Q K \<acute>CRB \<acute>buf_y  \<rbrace>, \<lbrace>True\<rbrace>"  
   by(oghoare, auto)  
 
+
 paragraph \<open>Incrementing the Tail Pointer\<close>
 
 text \<open>
@@ -4256,20 +4385,19 @@ text \<open>
 
 lemma  CleanQ_RB_incr_tail_x_hoare:
   "\<Gamma>, \<Theta> |\<turnstile>\<^bsub>/ F\<^esub>  
-    \<lbrace>  CleanQ_RB_deq_x_Q K \<acute>CRB b \<rbrace> 
-        \<acute>CRB := (CleanQ_RB_incr_tail_x b \<acute>CRB)
-    \<lbrace> CleanQ_RB_deq_x_R K \<acute>CRB b\<rbrace>,\<lbrace>True\<rbrace>" 
+  \<lbrace>  CleanQ_RB_deq_x_Q K \<acute>CRB b \<rbrace> 
+    \<acute>CRB := (CleanQ_RB_incr_tail_x b \<acute>CRB)
+  \<lbrace> CleanQ_RB_deq_x_R K \<acute>CRB b\<rbrace>,\<lbrace>True\<rbrace>" 
   by(oghoare, auto)
   
-
 lemma  CleanQ_RB_incr_tail_y_hoare:
-   "\<Gamma>, \<Theta> |\<turnstile>\<^bsub>/ F\<^esub> 
-    \<lbrace>  CleanQ_RB_deq_y_Q K \<acute>CRB b \<rbrace> 
-      \<acute>CRB := (CleanQ_RB_incr_tail_y b \<acute>CRB)
-    \<lbrace> CleanQ_RB_deq_y_R K \<acute> CRB b  \<rbrace>,\<lbrace>True\<rbrace>" 
+  "\<Gamma>, \<Theta> |\<turnstile>\<^bsub>/ F\<^esub> 
+  \<lbrace>  CleanQ_RB_deq_y_Q K \<acute>CRB b \<rbrace> 
+    \<acute>CRB := (CleanQ_RB_incr_tail_y b \<acute>CRB)
+  \<lbrace> CleanQ_RB_deq_y_R K \<acute> CRB b  \<rbrace>,\<lbrace>True\<rbrace>" 
   by(oghoare, auto)
 
- 
+
 paragraph \<open>Full Dequeue Operation\<close>
 
 text \<open>
@@ -4277,197 +4405,514 @@ text \<open>
 \<close>
 
 lemma CleanQ_RB_deq_x_hoare : 
-   "\<Gamma>, \<Theta> |\<turnstile>\<^bsub>/ F\<^esub>  
-    \<lbrace>  CleanQ_RB_deq_x_P K \<acute>CRB (CleanQ_RB_read_tail_x \<acute>CRB) \<rbrace> 
-      \<acute>buf_x := (CleanQ_RB_read_tail_x \<acute>CRB) ;;
-    \<lbrace> CleanQ_RB_deq_x_Q K \<acute>CRB \<acute>buf_x  \<rbrace>
-      \<acute>CRB := (CleanQ_RB_incr_tail_x \<acute>buf_x \<acute>CRB)
-    \<lbrace> CleanQ_RB_deq_x_R K \<acute>CRB \<acute>buf_x \<rbrace> , \<lbrace>True\<rbrace>"
+  "\<Gamma>, \<Theta> |\<turnstile>\<^bsub>/ F\<^esub>  
+  \<lbrace>  CleanQ_RB_deq_x_P K \<acute>CRB (CleanQ_RB_read_tail_x \<acute>CRB) \<rbrace> 
+    \<acute>buf_x := (CleanQ_RB_read_tail_x \<acute>CRB) ;;
+  \<lbrace> CleanQ_RB_deq_x_Q K \<acute>CRB \<acute>buf_x  \<rbrace>
+    \<acute>CRB := (CleanQ_RB_incr_tail_x \<acute>buf_x \<acute>CRB)
+  \<lbrace> CleanQ_RB_deq_x_R K \<acute>CRB \<acute>buf_x \<rbrace> , \<lbrace>True\<rbrace>"
   by(oghoare, auto)
-  
-  
   
 lemma CleanQ_RB_deq_y_hoare : 
-   "\<Gamma>, \<Theta> |\<turnstile>\<^bsub>/ F\<^esub>   
-    \<lbrace>  CleanQ_RB_deq_y_P K \<acute>CRB (CleanQ_RB_read_tail_x \<acute>CRB) \<rbrace> 
-      \<acute>buf_y := (CleanQ_RB_read_tail_y \<acute>CRB) ;;
-    \<lbrace> CleanQ_RB_deq_y_Q K \<acute>CRB \<acute>buf_y  \<rbrace>
-      \<acute>CRB := (CleanQ_RB_incr_tail_y \<acute>buf_y \<acute>CRB)
-    \<lbrace> CleanQ_RB_deq_y_R K \<acute>CRB \<acute>buf_y \<rbrace>, \<lbrace>True\<rbrace>"
-  by(oghoare, auto)
-  
-
-(* ------------------------------------------------------------------------------------ *)
-subsubsection \<open>Concurrency proofs helper lemmas\<close>
-(* ------------------------------------------------------------------------------------ *)
-
-(* ------------------------------------------------------------------------------------ *)
-subsubsection \<open>Concurrency proofs\<close>
-(* ------------------------------------------------------------------------------------ *)
-
-lemma CleanQ_RB_read_concurent:
-     "\<Gamma>, \<Theta> |\<turnstile>\<^bsub>/{True}\<^esub>   
-      COBEGIN
-         \<lbrace>  CleanQ_RB_Invariants \<acute>uni \<acute>CRB \<rbrace>
-           \<acute>buf_x := CleanQ_RB_read_head_x \<acute>CRB
-         \<lbrace>  CleanQ_RB_Invariants \<acute>uni \<acute>CRB \<rbrace>, \<lbrace>True\<rbrace>
-         \<parallel> 
-         \<lbrace>  CleanQ_RB_Invariants \<acute>uni \<acute>CRB \<rbrace>
-          \<acute>buf_y := CleanQ_RB_read_head_y \<acute>CRB
-         \<lbrace>  CleanQ_RB_Invariants \<acute>uni \<acute>CRB \<rbrace>, \<lbrace>True\<rbrace>
-      COEND
-      \<lbrace>  CleanQ_RB_Invariants \<acute>uni \<acute>CRB \<rbrace>, \<lbrace>True\<rbrace>"
+  "\<Gamma>, \<Theta> |\<turnstile>\<^bsub>/ F\<^esub>   
+  \<lbrace>  CleanQ_RB_deq_y_P K \<acute>CRB (CleanQ_RB_read_tail_x \<acute>CRB) \<rbrace> 
+    \<acute>buf_y := (CleanQ_RB_read_tail_y \<acute>CRB) ;;
+  \<lbrace> CleanQ_RB_deq_y_Q K \<acute>CRB \<acute>buf_y  \<rbrace>
+    \<acute>CRB := (CleanQ_RB_incr_tail_y \<acute>buf_y \<acute>CRB)
+  \<lbrace> CleanQ_RB_deq_y_R K \<acute>CRB \<acute>buf_y \<rbrace>, \<lbrace>True\<rbrace>"
   by(oghoare, auto)
 
-(* let's try this... I think we could start with this and showing this for all
-  four combinations. Then continue with splitting up *)
+text \<open>
+  Last we show that the \verb+dequeue+ operation in two steps is the same as the big 
+  step dequeue.
+\<close>
+
+lemma CleanQ_RB_deq_x_hoare_deq_equiv : 
+  "\<Gamma>, \<Theta> |\<turnstile>\<^bsub>/ F\<^esub>  
+  \<lbrace>  CleanQ_RB_deq_x_P K \<acute>CRB (CleanQ_RB_read_tail_x \<acute>CRB) \<and> rb = \<acute>CRB \<rbrace> 
+    \<acute>buf_x := (CleanQ_RB_read_tail_x \<acute>CRB) ;;
+  \<lbrace> CleanQ_RB_deq_x_Q K \<acute>CRB \<acute>buf_x \<and> rb = \<acute>CRB  \<rbrace>
+    \<acute>CRB := (CleanQ_RB_incr_tail_x \<acute>buf_x \<acute>CRB)
+  \<lbrace> CleanQ_RB_deq_x_R K \<acute>CRB \<acute>buf_x \<and> \<acute>CRB = CleanQ_RB_deq_x rb \<rbrace> , \<lbrace>True\<rbrace>"
+  by(oghoare, auto)
+
+lemma CleanQ_RB_deq_y_hoare_deq_equiv : 
+  "\<Gamma>, \<Theta> |\<turnstile>\<^bsub>/ F\<^esub>  
+  \<lbrace>  CleanQ_RB_deq_y_P K \<acute>CRB (CleanQ_RB_read_tail_y \<acute>CRB) \<and> rb = \<acute>CRB \<rbrace> 
+    \<acute>buf_y := (CleanQ_RB_read_tail_y \<acute>CRB) ;;
+  \<lbrace> CleanQ_RB_deq_y_Q K \<acute>CRB \<acute>buf_y \<and> rb = \<acute>CRB  \<rbrace>
+    \<acute>CRB := (CleanQ_RB_incr_tail_y \<acute>buf_y \<acute>CRB)
+  \<lbrace> CleanQ_RB_deq_y_R K \<acute>CRB \<acute>buf_y \<and> \<acute>CRB = CleanQ_RB_deq_y rb \<rbrace> , \<lbrace>True\<rbrace>"
+  by(oghoare, auto)
+
+
+paragraph \<open>Conditional Dequeue\<close>
+
+text \<open>
+  We now define the \verb+Dequeue+ operation as a convenient abbreviation, which 
+  includes the a conditional that checks if we can dequeue something. 
+\<close>
+
+abbreviation "CleanQ_CRB_deq_x \<equiv> 
+  \<lbrace> CleanQ_RB_Invariants \<acute>uni \<acute>CRB  \<rbrace>
+    IF CleanQ_RB_deq_x_possible \<acute>CRB
+    THEN
+      \<lbrace> CleanQ_RB_deq_x_P \<acute>uni \<acute>CRB (CleanQ_RB_read_tail_x \<acute>CRB) \<rbrace>
+        \<acute>buf_x := (CleanQ_RB_read_tail_x  \<acute>CRB) ;;
+      \<lbrace> CleanQ_RB_deq_x_Q \<acute>uni \<acute>CRB \<acute>buf_x \<rbrace>
+        \<acute>CRB := (CleanQ_RB_incr_tail_x \<acute>buf_x \<acute>CRB) ;;
+      \<lbrace> CleanQ_RB_deq_x_R \<acute>uni \<acute>CRB \<acute>buf_x \<rbrace>
+        SKIP
+    ELSE 
+      \<lbrace> CleanQ_RB_Invariants \<acute>uni \<acute>CRB \<rbrace>
+        SKIP
+    FI"
+
+
+abbreviation "CleanQ_CRB_deq_y \<equiv> 
+  \<lbrace> CleanQ_RB_Invariants \<acute>uni \<acute>CRB  \<rbrace>
+    IF CleanQ_RB_deq_y_possible \<acute>CRB
+    THEN
+      \<lbrace> CleanQ_RB_deq_y_P \<acute>uni \<acute>CRB (CleanQ_RB_read_tail_y \<acute>CRB) \<rbrace>
+        \<acute>buf_y := (CleanQ_RB_read_tail_y  \<acute>CRB) ;;
+      \<lbrace> CleanQ_RB_deq_y_Q \<acute>uni \<acute>CRB \<acute>buf_y \<rbrace>
+        \<acute>CRB := (CleanQ_RB_incr_tail_y \<acute>buf_y \<acute>CRB) ;;
+      \<lbrace> CleanQ_RB_deq_y_R \<acute>uni \<acute>CRB \<acute>buf_y \<rbrace>
+        SKIP
+    ELSE 
+      \<lbrace> CleanQ_RB_Invariants \<acute>uni \<acute>CRB \<rbrace>
+        SKIP
+    FI"
+
+
+paragraph \<open>Multistep Dequeue Operation\<close>
+
+text \<open>
+  Reading the entire record is not an atomic operation. So we define this as a sequence
+  of reading single fields in the record. 
+\<close>
+
+abbreviation "CleanQ_CRB_deq_mult_x \<equiv> 
+  \<lbrace> CleanQ_RB_Invariants \<acute>uni \<acute>CRB  \<rbrace>
+    IF CleanQ_RB_deq_x_possible \<acute>CRB
+    THEN
+      \<lbrace> CleanQ_RB_deq_x_P \<acute>uni \<acute>CRB (CleanQ_RB_read_tail_x \<acute>CRB) \<rbrace>
+        \<acute>buf_x := (CleanQ_RB_read_tail_region_x \<acute>CRB \<acute>buf_x) ;;
+      \<lbrace> CleanQ_RB_deq_x_P \<acute>uni \<acute>CRB (CleanQ_RB_read_tail_x \<acute>CRB) \<and>
+        \<acute>buf_x = CleanQ_RB_read_tail_region_x \<acute>CRB \<acute>buf_x
+      \<rbrace>
+        \<acute>buf_x := (CleanQ_RB_read_tail_offset_x \<acute>CRB \<acute>buf_x) ;;
+      \<lbrace> CleanQ_RB_deq_x_P \<acute>uni \<acute>CRB (CleanQ_RB_read_tail_x \<acute>CRB) \<and>
+        \<acute>buf_x = CleanQ_RB_read_tail_region_x \<acute>CRB \<acute>buf_x \<and>
+        \<acute>buf_x = CleanQ_RB_read_tail_offset_x \<acute>CRB \<acute>buf_x 
+      \<rbrace>
+        \<acute>buf_x := (CleanQ_RB_read_tail_length_x \<acute>CRB \<acute>buf_x) ;;
+      \<lbrace> CleanQ_RB_deq_x_P \<acute>uni \<acute>CRB (CleanQ_RB_read_tail_x \<acute>CRB) \<and>
+        \<acute>buf_x = CleanQ_RB_read_tail_region_x \<acute>CRB \<acute>buf_x \<and>
+        \<acute>buf_x = CleanQ_RB_read_tail_offset_x \<acute>CRB \<acute>buf_x \<and>
+        \<acute>buf_x = CleanQ_RB_read_tail_length_x \<acute>CRB \<acute>buf_x 
+      \<rbrace>
+        \<acute>buf_x := (CleanQ_RB_read_tail_valid_offset_x \<acute>CRB \<acute>buf_x) ;;
+      \<lbrace> CleanQ_RB_deq_x_P \<acute>uni \<acute>CRB (CleanQ_RB_read_tail_x \<acute>CRB) \<and>
+        \<acute>buf_x = CleanQ_RB_read_tail_region_x \<acute>CRB \<acute>buf_x \<and>
+        \<acute>buf_x = CleanQ_RB_read_tail_offset_x \<acute>CRB \<acute>buf_x \<and>
+        \<acute>buf_x = CleanQ_RB_read_tail_length_x \<acute>CRB \<acute>buf_x \<and>
+        \<acute>buf_x = CleanQ_RB_read_tail_valid_offset_x \<acute>CRB \<acute>buf_x 
+      \<rbrace>
+        \<acute>buf_x := (CleanQ_RB_read_tail_valid_length_x \<acute>CRB \<acute>buf_x) ;;
+      \<lbrace> CleanQ_RB_deq_x_P \<acute>uni \<acute>CRB (CleanQ_RB_read_tail_x \<acute>CRB) \<and>
+        \<acute>buf_x = CleanQ_RB_read_tail_region_x \<acute>CRB \<acute>buf_x \<and>
+        \<acute>buf_x = CleanQ_RB_read_tail_offset_x \<acute>CRB \<acute>buf_x \<and>
+        \<acute>buf_x = CleanQ_RB_read_tail_length_x \<acute>CRB \<acute>buf_x \<and>
+        \<acute>buf_x = CleanQ_RB_read_tail_valid_offset_x \<acute>CRB \<acute>buf_x \<and>
+        \<acute>buf_x = CleanQ_RB_read_tail_valid_length_x \<acute>CRB \<acute>buf_x 
+      \<rbrace>
+        \<acute>buf_x := (CleanQ_RB_read_tail_flags_x \<acute>CRB \<acute>buf_x) ;;
+      \<lbrace> CleanQ_RB_deq_x_Q \<acute>uni \<acute>CRB \<acute>buf_x\<rbrace>
+        \<acute>CRB := (CleanQ_RB_incr_tail_x \<acute>buf_x \<acute>CRB);;
+      \<lbrace> CleanQ_RB_deq_x_R \<acute>uni \<acute>CRB \<acute>buf_x \<rbrace>
+        SKIP
+    ELSE 
+      \<lbrace>  CleanQ_RB_Invariants \<acute>uni \<acute>CRB \<rbrace>
+      SKIP
+    FI"
+
+abbreviation "CleanQ_CRB_deq_mult_y \<equiv> 
+  \<lbrace> CleanQ_RB_Invariants \<acute>uni \<acute>CRB  \<rbrace>
+    IF CleanQ_RB_deq_y_possible \<acute>CRB
+    THEN
+      \<lbrace> CleanQ_RB_deq_y_P \<acute>uni \<acute>CRB (CleanQ_RB_read_tail_y \<acute>CRB) \<rbrace>
+        \<acute>buf_y := (CleanQ_RB_read_tail_region_y \<acute>CRB \<acute>buf_y) ;;
+      \<lbrace> CleanQ_RB_deq_y_P \<acute>uni \<acute>CRB (CleanQ_RB_read_tail_y \<acute>CRB) \<and>
+        \<acute>buf_y = CleanQ_RB_read_tail_region_y \<acute>CRB \<acute>buf_y
+      \<rbrace>
+        \<acute>buf_y := (CleanQ_RB_read_tail_offset_y \<acute>CRB \<acute>buf_y) ;;
+      \<lbrace> CleanQ_RB_deq_y_P \<acute>uni \<acute>CRB (CleanQ_RB_read_tail_y \<acute>CRB) \<and>
+        \<acute>buf_y = CleanQ_RB_read_tail_region_y \<acute>CRB \<acute>buf_y \<and>
+        \<acute>buf_y = CleanQ_RB_read_tail_offset_y \<acute>CRB \<acute>buf_y 
+      \<rbrace>
+        \<acute>buf_y := (CleanQ_RB_read_tail_length_y \<acute>CRB \<acute>buf_y) ;;
+      \<lbrace> CleanQ_RB_deq_y_P \<acute>uni \<acute>CRB (CleanQ_RB_read_tail_y \<acute>CRB) \<and>
+        \<acute>buf_y = CleanQ_RB_read_tail_region_y \<acute>CRB \<acute>buf_y \<and>
+        \<acute>buf_y = CleanQ_RB_read_tail_offset_y \<acute>CRB \<acute>buf_y \<and>
+        \<acute>buf_y = CleanQ_RB_read_tail_length_y \<acute>CRB \<acute>buf_y 
+      \<rbrace>
+        \<acute>buf_y := (CleanQ_RB_read_tail_valid_offset_y \<acute>CRB \<acute>buf_y) ;;
+      \<lbrace> CleanQ_RB_deq_y_P \<acute>uni \<acute>CRB (CleanQ_RB_read_tail_y \<acute>CRB) \<and>
+        \<acute>buf_y = CleanQ_RB_read_tail_region_y \<acute>CRB \<acute>buf_y \<and>
+        \<acute>buf_y = CleanQ_RB_read_tail_offset_y \<acute>CRB \<acute>buf_y \<and>
+        \<acute>buf_y = CleanQ_RB_read_tail_length_y \<acute>CRB \<acute>buf_y \<and>
+        \<acute>buf_y = CleanQ_RB_read_tail_valid_offset_y \<acute>CRB \<acute>buf_y 
+      \<rbrace>
+        \<acute>buf_y := (CleanQ_RB_read_tail_valid_length_y \<acute>CRB \<acute>buf_y) ;;
+      \<lbrace> CleanQ_RB_deq_y_P \<acute>uni \<acute>CRB (CleanQ_RB_read_tail_y \<acute>CRB) \<and>
+        \<acute>buf_y = CleanQ_RB_read_tail_region_y \<acute>CRB \<acute>buf_y \<and>
+        \<acute>buf_y = CleanQ_RB_read_tail_offset_y \<acute>CRB \<acute>buf_y \<and>
+        \<acute>buf_y = CleanQ_RB_read_tail_length_y \<acute>CRB \<acute>buf_y \<and>
+        \<acute>buf_y = CleanQ_RB_read_tail_valid_offset_y \<acute>CRB \<acute>buf_y \<and>
+        \<acute>buf_y = CleanQ_RB_read_tail_valid_length_y \<acute>CRB \<acute>buf_y 
+      \<rbrace>
+        \<acute>buf_y := (CleanQ_RB_read_tail_flags_y \<acute>CRB \<acute>buf_y) ;;
+      \<lbrace> CleanQ_RB_deq_y_Q \<acute>uni \<acute>CRB \<acute>buf_y\<rbrace>
+        \<acute>CRB := (CleanQ_RB_incr_tail_y \<acute>buf_y \<acute>CRB);;
+      \<lbrace> CleanQ_RB_deq_y_R \<acute>uni \<acute>CRB \<acute>buf_y \<rbrace>
+        SKIP
+    ELSE 
+      \<lbrace>  CleanQ_RB_Invariants \<acute>uni \<acute>CRB \<rbrace>
+      SKIP
+    FI"
+
+paragraph \<open>Also do the Conditional in MultiStep?\<close>
+
+text \<open>
+  Next, we expand the \verb+CleanQ_RB_deq_x|y_possible+ checks to expose those memory
+  accesses in the model. We first define the way to obtain the deq possible result.
+\<close>
+
+lemma CleanQ_RB_read_head_tail_deq_x_possible[simp]:
+  "CleanQ_RB_read_head_rx_x rb \<noteq> CleanQ_RB_read_tail_rx_x rb = CleanQ_RB_deq_x_possible rb"
+  by (simp add: CleanQ_RB_deq_x_possible_def CleanQ_RB_read_head_rx_x_def 
+                CleanQ_RB_read_tail_rx_x_def rb_can_deq_def rb_empty_def)
+
+lemma CleanQ_RB_read_head_tail_deq_y_possible[simp]:
+  "CleanQ_RB_read_head_rx_y rb \<noteq> CleanQ_RB_read_tail_rx_y rb = CleanQ_RB_deq_y_possible rb"
+  by (simp add: CleanQ_RB_deq_y_possible_def CleanQ_RB_read_head_rx_y_def 
+                CleanQ_RB_read_tail_rx_y_def rb_can_deq_def rb_empty_def)
+
+lemma CleanQ_RB_read_head_tail_deq_y_possible2[simp]:
+  "CleanQ_RB_read_tail_rx_y rb \<noteq> CleanQ_RB_read_head_rx_y rb = CleanQ_RB_deq_y_possible rb"
+  by (metis CleanQ_RB_read_head_tail_deq_y_possible)
+
+lemma CleanQ_RB_read_head_tail_deq_x_possible2[simp]:
+  "CleanQ_RB_read_tail_rx_x rb \<noteq> CleanQ_RB_read_head_rx_x rb = CleanQ_RB_deq_x_possible rb"
+  by (metis CleanQ_RB_read_head_tail_deq_x_possible)
+
+
+lemma CleanQ_RB_deq_possible_x_mult : 
+  "\<Gamma>, \<Theta> |\<turnstile>\<^bsub>/ F\<^esub>  
+  \<lbrace> CleanQ_RB_Invariants \<acute>uni \<acute>CRB \<rbrace> 
+    \<acute>head_x := CleanQ_RB_read_head_rx_x \<acute>CRB ;;
+  \<lbrace> \<acute>head_x = CleanQ_RB_read_head_rx_x \<acute>CRB \<rbrace>
+    \<acute>tail_x := CleanQ_RB_read_tail_rx_x \<acute>CRB
+  \<lbrace> (\<acute>tail_x \<noteq> \<acute>head_x) = CleanQ_RB_deq_x_possible \<acute>CRB  \<rbrace> , \<lbrace>True\<rbrace>"
+  apply(oghoare, auto)
+  by (metis CleanQ_RB_read_head_tail_deq_x_possible)
+
+lemma CleanQ_RB_deq_possible_y_mult : 
+  "\<Gamma>, \<Theta> |\<turnstile>\<^bsub>/ F\<^esub>  
+  \<lbrace> CleanQ_RB_Invariants \<acute>uni \<acute>CRB \<rbrace> 
+    \<acute>head_y := CleanQ_RB_read_head_rx_y \<acute>CRB ;;
+  \<lbrace> \<acute>head_y = CleanQ_RB_read_head_rx_y \<acute>CRB \<rbrace>
+    \<acute>tail_y := CleanQ_RB_read_tail_rx_y \<acute>CRB
+  \<lbrace> (\<acute>tail_y \<noteq> \<acute>head_y) = CleanQ_RB_deq_y_possible \<acute>CRB  \<rbrace> , \<lbrace>True\<rbrace>"
+  apply(oghoare, auto)
+  by (metis CleanQ_RB_read_head_tail_deq_y_possible)
+
+text \<open>
+
+\<close>
+
+(* *)
+
+abbreviation "CleanQ_CRB_deq_mult_if_x \<equiv> 
+  \<lbrace> CleanQ_RB_Invariants \<acute>uni \<acute>CRB  \<rbrace>
+    \<acute>tail_x := CleanQ_RB_read_tail_rx_x \<acute>CRB ;;
+  \<lbrace> CleanQ_RB_Invariants \<acute>uni \<acute>CRB  \<and> \<acute>tail_x = CleanQ_RB_read_tail_rx_x \<acute>CRB \<rbrace>
+   \<acute>head_x := CleanQ_RB_read_head_rx_x \<acute>CRB ;; 
+  \<lbrace> CleanQ_RB_Invariants \<acute>uni \<acute>CRB   \<and> \<acute>head_x = CleanQ_RB_read_head_rx_x \<acute>CRB \<and>
+     \<acute>tail_x = CleanQ_RB_read_tail_rx_x \<acute>CRB
+  \<rbrace>
+    IF (\<acute>tail_x \<noteq> \<acute>head_x)
+    THEN
+      \<lbrace> CleanQ_RB_deq_x_P \<acute>uni \<acute>CRB (CleanQ_RB_read_tail_x \<acute>CRB) \<rbrace>
+        \<acute>buf_x := (CleanQ_RB_read_tail_region_x \<acute>CRB \<acute>buf_x) ;;
+      \<lbrace> CleanQ_RB_deq_x_P \<acute>uni \<acute>CRB (CleanQ_RB_read_tail_x \<acute>CRB) \<and>
+        \<acute>buf_x = CleanQ_RB_read_tail_region_x \<acute>CRB \<acute>buf_x
+      \<rbrace>
+        \<acute>buf_x := (CleanQ_RB_read_tail_offset_x \<acute>CRB \<acute>buf_x) ;;
+      \<lbrace> CleanQ_RB_deq_x_P \<acute>uni \<acute>CRB (CleanQ_RB_read_tail_x \<acute>CRB) \<and>
+        \<acute>buf_x = CleanQ_RB_read_tail_region_x \<acute>CRB \<acute>buf_x \<and>
+        \<acute>buf_x = CleanQ_RB_read_tail_offset_x \<acute>CRB \<acute>buf_x 
+      \<rbrace>
+        \<acute>buf_x := (CleanQ_RB_read_tail_length_x \<acute>CRB \<acute>buf_x) ;;
+      \<lbrace> CleanQ_RB_deq_x_P \<acute>uni \<acute>CRB (CleanQ_RB_read_tail_x \<acute>CRB) \<and>
+        \<acute>buf_x = CleanQ_RB_read_tail_region_x \<acute>CRB \<acute>buf_x \<and>
+        \<acute>buf_x = CleanQ_RB_read_tail_offset_x \<acute>CRB \<acute>buf_x \<and>
+        \<acute>buf_x = CleanQ_RB_read_tail_length_x \<acute>CRB \<acute>buf_x 
+      \<rbrace>
+        \<acute>buf_x := (CleanQ_RB_read_tail_valid_offset_x \<acute>CRB \<acute>buf_x) ;;
+      \<lbrace> CleanQ_RB_deq_x_P \<acute>uni \<acute>CRB (CleanQ_RB_read_tail_x \<acute>CRB) \<and>
+        \<acute>buf_x = CleanQ_RB_read_tail_region_x \<acute>CRB \<acute>buf_x \<and>
+        \<acute>buf_x = CleanQ_RB_read_tail_offset_x \<acute>CRB \<acute>buf_x \<and>
+        \<acute>buf_x = CleanQ_RB_read_tail_length_x \<acute>CRB \<acute>buf_x \<and>
+        \<acute>buf_x = CleanQ_RB_read_tail_valid_offset_x \<acute>CRB \<acute>buf_x 
+      \<rbrace>
+        \<acute>buf_x := (CleanQ_RB_read_tail_valid_length_x \<acute>CRB \<acute>buf_x) ;;
+      \<lbrace> CleanQ_RB_deq_x_P \<acute>uni \<acute>CRB (CleanQ_RB_read_tail_x \<acute>CRB) \<and>
+        \<acute>buf_x = CleanQ_RB_read_tail_region_x \<acute>CRB \<acute>buf_x \<and>
+        \<acute>buf_x = CleanQ_RB_read_tail_offset_x \<acute>CRB \<acute>buf_x \<and>
+        \<acute>buf_x = CleanQ_RB_read_tail_length_x \<acute>CRB \<acute>buf_x \<and>
+        \<acute>buf_x = CleanQ_RB_read_tail_valid_offset_x \<acute>CRB \<acute>buf_x \<and>
+        \<acute>buf_x = CleanQ_RB_read_tail_valid_length_x \<acute>CRB \<acute>buf_x 
+      \<rbrace>
+        \<acute>buf_x := (CleanQ_RB_read_tail_flags_x \<acute>CRB \<acute>buf_x) ;;
+      \<lbrace> CleanQ_RB_deq_x_Q \<acute>uni \<acute>CRB \<acute>buf_x\<rbrace>
+        \<acute>CRB := (CleanQ_RB_incr_tail_x \<acute>buf_x \<acute>CRB);;
+      \<lbrace> CleanQ_RB_deq_x_R \<acute>uni \<acute>CRB \<acute>buf_x \<rbrace>
+        SKIP
+    ELSE 
+      \<lbrace>  CleanQ_RB_Invariants \<acute>uni \<acute>CRB \<rbrace>
+      SKIP
+    FI"
+
+abbreviation "CleanQ_CRB_deq_mult_if_y \<equiv> 
+  \<lbrace> CleanQ_RB_Invariants \<acute>uni \<acute>CRB  \<rbrace>
+    \<acute>tail_y := CleanQ_RB_read_tail_rx_y \<acute>CRB ;;
+  \<lbrace> CleanQ_RB_Invariants \<acute>uni \<acute>CRB  \<and> \<acute>tail_y = CleanQ_RB_read_tail_rx_y \<acute>CRB \<rbrace>
+   \<acute>head_y := CleanQ_RB_read_head_rx_y \<acute>CRB ;; 
+ \<lbrace> CleanQ_RB_Invariants \<acute>uni \<acute>CRB  \<and> \<acute>head_y = CleanQ_RB_read_head_rx_y \<acute>CRB \<and>
+    \<acute>tail_y = CleanQ_RB_read_tail_rx_y \<acute>CRB 
+  \<rbrace>
+    IF (\<acute>tail_y \<noteq> \<acute>head_y)  
+    THEN
+      \<lbrace> CleanQ_RB_deq_y_P \<acute>uni \<acute>CRB (CleanQ_RB_read_tail_y \<acute>CRB) \<rbrace>
+        \<acute>buf_y := (CleanQ_RB_read_tail_region_y \<acute>CRB \<acute>buf_y) ;;
+      \<lbrace> CleanQ_RB_deq_y_P \<acute>uni \<acute>CRB (CleanQ_RB_read_tail_y \<acute>CRB) \<and>
+        \<acute>buf_y = CleanQ_RB_read_tail_region_y \<acute>CRB \<acute>buf_y
+      \<rbrace>
+        \<acute>buf_y := (CleanQ_RB_read_tail_offset_y \<acute>CRB \<acute>buf_y) ;;
+      \<lbrace> CleanQ_RB_deq_y_P \<acute>uni \<acute>CRB (CleanQ_RB_read_tail_y \<acute>CRB) \<and>
+        \<acute>buf_y = CleanQ_RB_read_tail_region_y \<acute>CRB \<acute>buf_y \<and>
+        \<acute>buf_y = CleanQ_RB_read_tail_offset_y \<acute>CRB \<acute>buf_y 
+      \<rbrace>
+        \<acute>buf_y := (CleanQ_RB_read_tail_length_y \<acute>CRB \<acute>buf_y) ;;
+      \<lbrace> CleanQ_RB_deq_y_P \<acute>uni \<acute>CRB (CleanQ_RB_read_tail_y \<acute>CRB) \<and>
+        \<acute>buf_y = CleanQ_RB_read_tail_region_y \<acute>CRB \<acute>buf_y \<and>
+        \<acute>buf_y = CleanQ_RB_read_tail_offset_y \<acute>CRB \<acute>buf_y \<and>
+        \<acute>buf_y = CleanQ_RB_read_tail_length_y \<acute>CRB \<acute>buf_y 
+      \<rbrace>
+        \<acute>buf_y := (CleanQ_RB_read_tail_valid_offset_y \<acute>CRB \<acute>buf_y) ;;
+      \<lbrace> CleanQ_RB_deq_y_P \<acute>uni \<acute>CRB (CleanQ_RB_read_tail_y \<acute>CRB) \<and>
+        \<acute>buf_y = CleanQ_RB_read_tail_region_y \<acute>CRB \<acute>buf_y \<and>
+        \<acute>buf_y = CleanQ_RB_read_tail_offset_y \<acute>CRB \<acute>buf_y \<and>
+        \<acute>buf_y = CleanQ_RB_read_tail_length_y \<acute>CRB \<acute>buf_y \<and>
+        \<acute>buf_y = CleanQ_RB_read_tail_valid_offset_y \<acute>CRB \<acute>buf_y 
+      \<rbrace>
+        \<acute>buf_y := (CleanQ_RB_read_tail_valid_length_y \<acute>CRB \<acute>buf_y) ;;
+      \<lbrace> CleanQ_RB_deq_y_P \<acute>uni \<acute>CRB (CleanQ_RB_read_tail_y \<acute>CRB) \<and>
+        \<acute>buf_y = CleanQ_RB_read_tail_region_y \<acute>CRB \<acute>buf_y \<and>
+        \<acute>buf_y = CleanQ_RB_read_tail_offset_y \<acute>CRB \<acute>buf_y \<and>
+        \<acute>buf_y = CleanQ_RB_read_tail_length_y \<acute>CRB \<acute>buf_y \<and>
+        \<acute>buf_y = CleanQ_RB_read_tail_valid_offset_y \<acute>CRB \<acute>buf_y \<and>
+        \<acute>buf_y = CleanQ_RB_read_tail_valid_length_y \<acute>CRB \<acute>buf_y 
+      \<rbrace>
+        \<acute>buf_y := (CleanQ_RB_read_tail_flags_y \<acute>CRB \<acute>buf_y) ;;
+      \<lbrace> CleanQ_RB_deq_y_Q \<acute>uni \<acute>CRB \<acute>buf_y\<rbrace>
+        \<acute>CRB := (CleanQ_RB_incr_tail_y \<acute>buf_y \<acute>CRB);;
+      \<lbrace> CleanQ_RB_deq_y_R \<acute>uni \<acute>CRB \<acute>buf_y \<rbrace>
+        SKIP
+    ELSE 
+      \<lbrace>  CleanQ_RB_Invariants \<acute>uni \<acute>CRB \<rbrace>
+      SKIP
+    FI"
+
+(* ==================================================================================== *)
+subsection \<open>Concurrency proofs\<close>
+(* ==================================================================================== *)
+
+paragraph\<open>Big Step Semantics\<close>
+
+text \<open>
+  We first start of using the big-step semantics for enqueue and dequeue. 
+\<close>
 
 lemma CleanQ_RB_loop_enq_enq:
-     "\<Gamma>, \<Theta> |\<turnstile>\<^bsub>/{True}\<^esub>   
-      COBEGIN
-         \<lbrace>  CleanQ_RB_Invariants \<acute>uni \<acute>CRB \<rbrace>
-         WHILE True INV \<lbrace>  CleanQ_RB_Invariants \<acute>uni \<acute>CRB \<rbrace>
-         DO \<lbrace>  CleanQ_RB_Invariants \<acute>uni \<acute>CRB \<rbrace>
-           (True,\<lbrace> CleanQ_RB_enq_x_P \<acute>uni \<acute>CRB bx \<rbrace>) \<longmapsto> 
-           \<lbrace>  CleanQ_RB_enq_x_P \<acute>uni \<acute>CRB bx \<rbrace>
-          \<acute>CRB := CleanQ_RB_enq_x bx \<acute>CRB
-         OD
-         \<lbrace>  CleanQ_RB_enq_x_R \<acute>uni \<acute>CRB bx \<rbrace>, \<lbrace>True\<rbrace>  
-         \<parallel> 
-         \<lbrace>  CleanQ_RB_Invariants \<acute>uni \<acute>CRB \<rbrace>
-         WHILE True INV \<lbrace>  CleanQ_RB_Invariants \<acute>uni \<acute>CRB \<rbrace>
-         DO
-        \<lbrace>  CleanQ_RB_Invariants \<acute>uni \<acute>CRB \<rbrace>
-          (True, \<lbrace>  CleanQ_RB_enq_y_P \<acute>uni \<acute>CRB by \<rbrace>) \<longmapsto> 
-            \<lbrace>  CleanQ_RB_enq_y_P \<acute>uni \<acute>CRB by \<rbrace>
-            \<acute>CRB := CleanQ_RB_enq_y by \<acute>CRB
-         OD
-         \<lbrace>  CleanQ_RB_enq_y_R \<acute>uni \<acute>CRB by \<rbrace>, \<lbrace>True\<rbrace>
-      COEND
-      \<lbrace>  CleanQ_RB_Invariants \<acute>uni \<acute>CRB \<rbrace>, \<lbrace>True\<rbrace>"
-  by(oghoare, auto)
-
-  
+  "\<Gamma>, \<Theta> |\<turnstile>\<^bsub>/{True}\<^esub>   
+  COBEGIN
+    \<lbrace>  CleanQ_RB_Invariants \<acute>uni \<acute>CRB \<rbrace>
+    WHILE True INV \<lbrace>  CleanQ_RB_Invariants \<acute>uni \<acute>CRB \<rbrace>
+    DO \<lbrace>  CleanQ_RB_Invariants \<acute>uni \<acute>CRB \<rbrace>
+      (True,\<lbrace> CleanQ_RB_enq_x_P \<acute>uni \<acute>CRB bx \<rbrace>) \<longmapsto> 
+      \<lbrace>  CleanQ_RB_enq_x_P \<acute>uni \<acute>CRB bx \<rbrace>
+      \<acute>CRB := CleanQ_RB_enq_x bx \<acute>CRB
+    OD
+    \<lbrace>  CleanQ_RB_enq_x_R \<acute>uni \<acute>CRB bx \<rbrace>, \<lbrace>True\<rbrace>  
+  \<parallel> 
+    \<lbrace>  CleanQ_RB_Invariants \<acute>uni \<acute>CRB \<rbrace>
+    WHILE True INV \<lbrace>  CleanQ_RB_Invariants \<acute>uni \<acute>CRB \<rbrace>
+    DO
+      \<lbrace>  CleanQ_RB_Invariants \<acute>uni \<acute>CRB \<rbrace>
+      (True, \<lbrace>  CleanQ_RB_enq_y_P \<acute>uni \<acute>CRB by \<rbrace>) \<longmapsto> 
+      \<lbrace>  CleanQ_RB_enq_y_P \<acute>uni \<acute>CRB by \<rbrace>
+      \<acute>CRB := CleanQ_RB_enq_y by \<acute>CRB
+    OD
+    \<lbrace>  CleanQ_RB_enq_y_R \<acute>uni \<acute>CRB by \<rbrace>, \<lbrace>True\<rbrace>
+  COEND
+  \<lbrace> CleanQ_RB_Invariants \<acute>uni \<acute>CRB \<rbrace>, \<lbrace>True\<rbrace>"
+  by(oghoare, auto) 
   
 lemma CleanQ_RB_loop_enq_deq:
-     "\<Gamma>, \<Theta> |\<turnstile>\<^bsub>/{True}\<^esub>   
-      COBEGIN
-         \<lbrace>  CleanQ_RB_Invariants \<acute>uni \<acute>CRB \<rbrace>
-         WHILE True INV \<lbrace>  CleanQ_RB_Invariants \<acute>uni \<acute>CRB \<rbrace>
-         DO \<lbrace>  CleanQ_RB_Invariants \<acute>uni \<acute>CRB \<rbrace>
-           (True,\<lbrace> CleanQ_RB_enq_x_P \<acute>uni \<acute>CRB bx \<rbrace>) \<longmapsto> 
-           \<lbrace>  CleanQ_RB_enq_x_P \<acute>uni \<acute>CRB bx \<rbrace>
-          \<acute>CRB := CleanQ_RB_enq_x bx \<acute>CRB
-         OD
-         \<lbrace>  CleanQ_RB_enq_x_R \<acute>uni \<acute>CRB bx \<rbrace>, \<lbrace>True\<rbrace>  
-         \<parallel> 
-         \<lbrace>  CleanQ_RB_Invariants \<acute>uni \<acute>CRB \<rbrace>
-         WHILE True INV \<lbrace>  CleanQ_RB_Invariants \<acute>uni \<acute>CRB \<rbrace>
-         DO
-        \<lbrace>  CleanQ_RB_Invariants \<acute>uni \<acute>CRB \<rbrace>
-          (True, \<lbrace>  CleanQ_RB_deq_y_P \<acute>uni \<acute>CRB by \<rbrace>) \<longmapsto> 
-            \<lbrace>  CleanQ_RB_deq_y_P \<acute>uni \<acute>CRB by \<rbrace>
-            \<acute>CRB := CleanQ_RB_deq_y \<acute>CRB
-         OD
-         \<lbrace>  CleanQ_RB_deq_y_R \<acute>uni \<acute>CRB by \<rbrace>, \<lbrace>True\<rbrace>
-      COEND
-      \<lbrace>  CleanQ_RB_Invariants \<acute>uni \<acute>CRB \<rbrace>, \<lbrace>True\<rbrace>"
+  "\<Gamma>, \<Theta> |\<turnstile>\<^bsub>/{True}\<^esub>   
+  COBEGIN
+    \<lbrace>  CleanQ_RB_Invariants \<acute>uni \<acute>CRB \<rbrace>
+    WHILE True INV \<lbrace>  CleanQ_RB_Invariants \<acute>uni \<acute>CRB \<rbrace>
+    DO \<lbrace>  CleanQ_RB_Invariants \<acute>uni \<acute>CRB \<rbrace>
+      (True,\<lbrace> CleanQ_RB_enq_x_P \<acute>uni \<acute>CRB bx \<rbrace>) \<longmapsto> 
+      \<lbrace>  CleanQ_RB_enq_x_P \<acute>uni \<acute>CRB bx \<rbrace>
+      \<acute>CRB := CleanQ_RB_enq_x bx \<acute>CRB
+    OD
+    \<lbrace>  CleanQ_RB_enq_x_R \<acute>uni \<acute>CRB bx \<rbrace>, \<lbrace>True\<rbrace>  
+  \<parallel> 
+    \<lbrace>  CleanQ_RB_Invariants \<acute>uni \<acute>CRB \<rbrace>
+    WHILE True INV \<lbrace>  CleanQ_RB_Invariants \<acute>uni \<acute>CRB \<rbrace>
+    DO
+      \<lbrace>  CleanQ_RB_Invariants \<acute>uni \<acute>CRB \<rbrace>
+      (True, \<lbrace>  CleanQ_RB_deq_y_P \<acute>uni \<acute>CRB by \<rbrace>) \<longmapsto> 
+      \<lbrace>  CleanQ_RB_deq_y_P \<acute>uni \<acute>CRB by \<rbrace>
+      \<acute>CRB := CleanQ_RB_deq_y \<acute>CRB
+    OD
+    \<lbrace>  CleanQ_RB_deq_y_R \<acute>uni \<acute>CRB by \<rbrace>, \<lbrace>True\<rbrace>
+  COEND
+  \<lbrace>  CleanQ_RB_Invariants \<acute>uni \<acute>CRB \<rbrace>, \<lbrace>True\<rbrace>"
   by(oghoare, auto)
 
 lemma CleanQ_RB_loop_deq_enq:
-     "\<Gamma>, \<Theta> |\<turnstile>\<^bsub>/{True}\<^esub>   
-      COBEGIN
-         \<lbrace>  CleanQ_RB_Invariants \<acute>uni \<acute>CRB \<rbrace>
-         WHILE True INV \<lbrace>  CleanQ_RB_Invariants \<acute>uni \<acute>CRB \<rbrace>
-         DO \<lbrace>  CleanQ_RB_Invariants \<acute>uni \<acute>CRB \<rbrace>
-           (True,\<lbrace> CleanQ_RB_deq_x_P \<acute>uni \<acute>CRB bx \<rbrace>) \<longmapsto> 
-           \<lbrace>  CleanQ_RB_deq_x_P \<acute>uni \<acute>CRB bx \<rbrace>
-          \<acute>CRB := CleanQ_RB_deq_x \<acute>CRB
-         OD
-         \<lbrace>  CleanQ_RB_deq_x_R \<acute>uni \<acute>CRB bx \<rbrace>, \<lbrace>True\<rbrace>  
-         \<parallel> 
-         \<lbrace>  CleanQ_RB_Invariants \<acute>uni \<acute>CRB \<rbrace>
-         WHILE True INV \<lbrace>  CleanQ_RB_Invariants \<acute>uni \<acute>CRB \<rbrace>
-         DO
-        \<lbrace>  CleanQ_RB_Invariants \<acute>uni \<acute>CRB \<rbrace>
-          (True, \<lbrace>  CleanQ_RB_enq_y_P \<acute>uni \<acute>CRB by \<rbrace>) \<longmapsto> 
-            \<lbrace>  CleanQ_RB_enq_y_P \<acute>uni \<acute>CRB by \<rbrace>
-            \<acute>CRB := CleanQ_RB_enq_y by \<acute>CRB 
-         OD
-         \<lbrace>  CleanQ_RB_enq_y_R \<acute>uni \<acute>CRB by \<rbrace>, \<lbrace>True\<rbrace>
-      COEND
-      \<lbrace>  CleanQ_RB_Invariants \<acute>uni \<acute>CRB \<rbrace>, \<lbrace>True\<rbrace>" 
+  "\<Gamma>, \<Theta> |\<turnstile>\<^bsub>/{True}\<^esub>   
+  COBEGIN
+    \<lbrace>  CleanQ_RB_Invariants \<acute>uni \<acute>CRB \<rbrace>
+    WHILE True INV \<lbrace>  CleanQ_RB_Invariants \<acute>uni \<acute>CRB \<rbrace>
+    DO \<lbrace>  CleanQ_RB_Invariants \<acute>uni \<acute>CRB \<rbrace>
+      (True,\<lbrace> CleanQ_RB_deq_x_P \<acute>uni \<acute>CRB bx \<rbrace>) \<longmapsto> 
+      \<lbrace>  CleanQ_RB_deq_x_P \<acute>uni \<acute>CRB bx \<rbrace>
+     \<acute>CRB := CleanQ_RB_deq_x \<acute>CRB
+    OD
+    \<lbrace>  CleanQ_RB_deq_x_R \<acute>uni \<acute>CRB bx \<rbrace>, \<lbrace>True\<rbrace>  
+  \<parallel> 
+    \<lbrace>  CleanQ_RB_Invariants \<acute>uni \<acute>CRB \<rbrace>
+    WHILE True INV \<lbrace>  CleanQ_RB_Invariants \<acute>uni \<acute>CRB \<rbrace>
+    DO
+      \<lbrace>  CleanQ_RB_Invariants \<acute>uni \<acute>CRB \<rbrace>
+      (True, \<lbrace>  CleanQ_RB_enq_y_P \<acute>uni \<acute>CRB by \<rbrace>) \<longmapsto> 
+      \<lbrace>  CleanQ_RB_enq_y_P \<acute>uni \<acute>CRB by \<rbrace>
+      \<acute>CRB := CleanQ_RB_enq_y by \<acute>CRB 
+    OD
+    \<lbrace>  CleanQ_RB_enq_y_R \<acute>uni \<acute>CRB by \<rbrace>, \<lbrace>True\<rbrace>
+  COEND
+  \<lbrace>  CleanQ_RB_Invariants \<acute>uni \<acute>CRB \<rbrace>, \<lbrace>True\<rbrace>" 
  by(oghoare, auto)
   
     
- lemma CleanQ_RB_loop_deq_deq:
-     "\<Gamma>, \<Theta> |\<turnstile>\<^bsub>/{True}\<^esub>   
-      COBEGIN
-         \<lbrace>  CleanQ_RB_Invariants \<acute>uni \<acute>CRB \<rbrace>
-         WHILE True INV \<lbrace>  CleanQ_RB_Invariants \<acute>uni \<acute>CRB \<rbrace>
-         DO \<lbrace>  CleanQ_RB_Invariants \<acute>uni \<acute>CRB \<rbrace>
-           (True,\<lbrace> CleanQ_RB_deq_x_P \<acute>uni \<acute>CRB (CleanQ_RB_read_tail_x \<acute>CRB) \<rbrace>) \<longmapsto> 
-           \<lbrace>  CleanQ_RB_deq_x_P \<acute>uni \<acute>CRB (CleanQ_RB_read_tail_x \<acute>CRB)  \<rbrace>
-          \<acute>CRB := CleanQ_RB_deq_x \<acute>CRB
-         OD
-         \<lbrace>  CleanQ_RB_deq_x_R \<acute>uni \<acute>CRB \<acute>buf_x \<rbrace>, \<lbrace>True\<rbrace>  
-         \<parallel> 
-         \<lbrace>  CleanQ_RB_Invariants \<acute>uni \<acute>CRB \<rbrace>
-         WHILE True INV \<lbrace>  CleanQ_RB_Invariants \<acute>uni \<acute>CRB \<rbrace>
-         DO
-        \<lbrace>  CleanQ_RB_Invariants \<acute>uni \<acute>CRB \<rbrace>
-          (True, \<lbrace>  CleanQ_RB_deq_y_P \<acute>uni \<acute>CRB (CleanQ_RB_read_tail_x \<acute>CRB) \<rbrace>) \<longmapsto> 
-            \<lbrace>  CleanQ_RB_deq_y_P \<acute>uni \<acute>CRB (CleanQ_RB_read_tail_x \<acute>CRB) \<rbrace>
-            \<acute>CRB := CleanQ_RB_deq_y \<acute>CRB 
-         OD
-         \<lbrace>  CleanQ_RB_deq_y_R \<acute>uni \<acute>CRB \<acute>buf_y \<rbrace>, \<lbrace>True\<rbrace>
-      COEND
-      \<lbrace>  CleanQ_RB_Invariants \<acute>uni \<acute>CRB \<rbrace>, \<lbrace>True\<rbrace>" 
-   by(oghoare, auto)
-   
-  
-  
+lemma CleanQ_RB_loop_deq_deq:
+  "\<Gamma>, \<Theta> |\<turnstile>\<^bsub>/{True}\<^esub>   
+  COBEGIN
+    \<lbrace>  CleanQ_RB_Invariants \<acute>uni \<acute>CRB \<rbrace>
+    WHILE True INV \<lbrace>  CleanQ_RB_Invariants \<acute>uni \<acute>CRB \<rbrace>
+    DO 
+      \<lbrace> CleanQ_RB_Invariants \<acute>uni \<acute>CRB \<rbrace>
+      (True,\<lbrace> CleanQ_RB_deq_x_P \<acute>uni \<acute>CRB (CleanQ_RB_read_tail_x \<acute>CRB) \<rbrace>) \<longmapsto> 
+      \<lbrace>  CleanQ_RB_deq_x_P \<acute>uni \<acute>CRB (CleanQ_RB_read_tail_x \<acute>CRB)  \<rbrace>
+      \<acute>CRB := CleanQ_RB_deq_x \<acute>CRB
+      OD
+    \<lbrace>  CleanQ_RB_deq_x_R \<acute>uni \<acute>CRB \<acute>buf_x \<rbrace>, \<lbrace>True\<rbrace>  
+  \<parallel> 
+    \<lbrace>  CleanQ_RB_Invariants \<acute>uni \<acute>CRB \<rbrace>
+    WHILE True INV \<lbrace>  CleanQ_RB_Invariants \<acute>uni \<acute>CRB \<rbrace>
+    DO
+      \<lbrace>  CleanQ_RB_Invariants \<acute>uni \<acute>CRB \<rbrace>
+      (True, \<lbrace>  CleanQ_RB_deq_y_P \<acute>uni \<acute>CRB (CleanQ_RB_read_tail_x \<acute>CRB) \<rbrace>) \<longmapsto> 
+      \<lbrace>  CleanQ_RB_deq_y_P \<acute>uni \<acute>CRB (CleanQ_RB_read_tail_x \<acute>CRB) \<rbrace>
+      \<acute>CRB := CleanQ_RB_deq_y \<acute>CRB 
+    OD
+    \<lbrace>  CleanQ_RB_deq_y_R \<acute>uni \<acute>CRB \<acute>buf_y \<rbrace>, \<lbrace>True\<rbrace>
+  COEND
+  \<lbrace>  CleanQ_RB_Invariants \<acute>uni \<acute>CRB \<rbrace>, \<lbrace>True\<rbrace>" 
+by(oghoare, auto)
+
+paragraph\<open>Breaking Up Into Update Buffer, Increment Pointers\<close>
+
+text \<open>
+  We now show that using guarded statements and breaking up the enqueue and dequeue
+  operations into buffer read/write and head/tail increment still yields the correct
+  semantics.
+\<close>
+
+
+
 lemma CleanQ_RB_concurrent_all:
-     "\<Gamma>, \<Theta> |\<turnstile>\<^bsub>/{True}\<^esub>   
-      COBEGIN
-         \<lbrace>  CleanQ_RB_Invariants \<acute>uni \<acute>CRB \<rbrace>
-         WHILE True INV \<lbrace>  CleanQ_RB_Invariants \<acute>uni \<acute>CRB \<rbrace>
-         DO \<lbrace>  CleanQ_RB_Invariants \<acute>uni \<acute>CRB \<rbrace>
-              (True, \<lbrace> CleanQ_RB_enq_x_P \<acute>uni \<acute>CRB bx \<rbrace>) \<longmapsto> ( 
-            \<lbrace> CleanQ_RB_enq_x_P \<acute>uni \<acute>CRB bx \<rbrace>
-              \<acute>CRB := (CleanQ_RB_write_head_x bx \<acute>CRB) ;;
-            \<lbrace> CleanQ_RB_enq_x_Q \<acute>uni \<acute>CRB bx \<rbrace>
-              \<acute>CRB := (CleanQ_RB_incr_head_x bx \<acute>CRB)) ;;
-            \<lbrace>  CleanQ_RB_Invariants \<acute>uni \<acute>CRB \<rbrace>
-              (True,\<lbrace> CleanQ_RB_deq_x_P \<acute>uni \<acute>CRB (CleanQ_RB_read_tail_x \<acute>CRB) \<rbrace>) \<longmapsto> ( 
-            \<lbrace> CleanQ_RB_deq_x_P \<acute>uni \<acute>CRB (CleanQ_RB_read_tail_x \<acute>CRB) \<rbrace>
-              \<acute>buf_x := (CleanQ_RB_read_tail_x \<acute>CRB) ;;
-            \<lbrace> CleanQ_RB_deq_x_Q \<acute>uni \<acute>CRB \<acute>buf_x \<rbrace>
-             \<acute>CRB := (CleanQ_RB_incr_tail_x \<acute>buf_x \<acute>CRB))
-         OD
-         \<lbrace>  CleanQ_RB_deq_x_R \<acute>uni \<acute>CRB \<acute>buf_x \<rbrace>, \<lbrace>True\<rbrace>  
-         \<parallel> 
-         \<lbrace>  CleanQ_RB_Invariants \<acute>uni \<acute>CRB \<rbrace>
-         WHILE True INV \<lbrace>  CleanQ_RB_Invariants \<acute>uni \<acute>CRB \<rbrace>
-         DO \<lbrace>  CleanQ_RB_Invariants \<acute>uni \<acute>CRB \<rbrace>
-              (True, \<lbrace> CleanQ_RB_enq_y_P \<acute>uni \<acute>CRB by \<rbrace>) \<longmapsto> ( 
-            \<lbrace> CleanQ_RB_enq_y_P \<acute>uni \<acute>CRB by \<rbrace>
-              \<acute>CRB := (CleanQ_RB_write_head_y by \<acute>CRB) ;;
-            \<lbrace> CleanQ_RB_enq_y_Q \<acute>uni \<acute>CRB by \<rbrace>
-              \<acute>CRB := (CleanQ_RB_incr_head_y by \<acute>CRB)) ;;
-            \<lbrace>  CleanQ_RB_Invariants \<acute>uni \<acute>CRB \<rbrace>
-              (True,\<lbrace> CleanQ_RB_deq_y_P \<acute>uni \<acute>CRB (CleanQ_RB_read_tail_y \<acute>CRB) \<rbrace>) \<longmapsto> ( 
-            \<lbrace> CleanQ_RB_deq_y_P \<acute>uni \<acute>CRB (CleanQ_RB_read_tail_y \<acute>CRB) \<rbrace>
-              \<acute>buf_y := (CleanQ_RB_read_tail_y \<acute>CRB) ;;
-            \<lbrace> CleanQ_RB_deq_y_Q \<acute>uni \<acute>CRB \<acute>buf_y \<rbrace>
-             \<acute>CRB := (CleanQ_RB_incr_tail_y \<acute>buf_y \<acute>CRB))
-         OD
-         \<lbrace>  CleanQ_RB_deq_y_R \<acute>uni \<acute>CRB \<acute>buf_y \<rbrace>, \<lbrace>True\<rbrace>
-      COEND
-      \<lbrace>  CleanQ_RB_Invariants \<acute>uni \<acute>CRB \<rbrace>, \<lbrace>True\<rbrace>" 
+  "\<Gamma>, \<Theta> |\<turnstile>\<^bsub>/{True}\<^esub>   
+  COBEGIN
+    \<lbrace>  CleanQ_RB_Invariants \<acute>uni \<acute>CRB \<rbrace>
+    WHILE True INV \<lbrace>  CleanQ_RB_Invariants \<acute>uni \<acute>CRB \<rbrace>
+    DO 
+      \<lbrace> CleanQ_RB_Invariants \<acute>uni \<acute>CRB \<rbrace>
+      (True, \<lbrace> CleanQ_RB_enq_x_P \<acute>uni \<acute>CRB bx \<rbrace>) \<longmapsto> ( 
+        \<lbrace> CleanQ_RB_enq_x_P \<acute>uni \<acute>CRB bx \<rbrace>
+        \<acute>CRB := (CleanQ_RB_write_head_x bx \<acute>CRB) ;;
+        \<lbrace> CleanQ_RB_enq_x_Q \<acute>uni \<acute>CRB bx \<rbrace>
+        \<acute>CRB := (CleanQ_RB_incr_head_x bx \<acute>CRB) ;;
+        \<lbrace> CleanQ_RB_enq_x_R \<acute>uni \<acute>CRB bx \<rbrace>
+        SKIP);;
+      \<lbrace> CleanQ_RB_Invariants \<acute>uni \<acute>CRB \<rbrace>
+      (True,\<lbrace> CleanQ_RB_deq_x_P \<acute>uni \<acute>CRB (CleanQ_RB_read_tail_x \<acute>CRB) \<rbrace>) \<longmapsto> ( 
+        \<lbrace> CleanQ_RB_deq_x_P \<acute>uni \<acute>CRB (CleanQ_RB_read_tail_x \<acute>CRB) \<rbrace>
+        \<acute>buf_x := (CleanQ_RB_read_tail_x \<acute>CRB) ;;
+        \<lbrace> CleanQ_RB_deq_x_Q \<acute>uni \<acute>CRB \<acute>buf_x \<rbrace>
+        \<acute>CRB := (CleanQ_RB_incr_tail_x \<acute>buf_x \<acute>CRB) ;;
+        \<lbrace> CleanQ_RB_deq_x_R \<acute>uni \<acute>CRB \<acute>buf_x \<rbrace>
+        SKIP)
+    OD
+    \<lbrace> CleanQ_RB_Invariants \<acute>uni \<acute>CRB \<rbrace>, \<lbrace>True\<rbrace>  
+  \<parallel> 
+    \<lbrace>  CleanQ_RB_Invariants \<acute>uni \<acute>CRB \<rbrace>
+    WHILE True INV \<lbrace>  CleanQ_RB_Invariants \<acute>uni \<acute>CRB \<rbrace>
+    DO 
+      \<lbrace> CleanQ_RB_Invariants \<acute>uni \<acute>CRB \<rbrace>
+      (True, \<lbrace> CleanQ_RB_enq_y_P \<acute>uni \<acute>CRB by \<rbrace>) \<longmapsto> ( 
+        \<lbrace> CleanQ_RB_enq_y_P \<acute>uni \<acute>CRB by \<rbrace>
+        \<acute>CRB := (CleanQ_RB_write_head_y by \<acute>CRB) ;;
+        \<lbrace> CleanQ_RB_enq_y_Q \<acute>uni \<acute>CRB by \<rbrace>
+        \<acute>CRB := (CleanQ_RB_incr_head_y by \<acute>CRB) ;;
+        \<lbrace>  CleanQ_RB_enq_y_R \<acute>uni \<acute>CRB by \<rbrace>
+        SKIP);;
+      \<lbrace> CleanQ_RB_Invariants \<acute>uni \<acute>CRB \<rbrace>
+      (True,\<lbrace> CleanQ_RB_deq_y_P \<acute>uni \<acute>CRB (CleanQ_RB_read_tail_y \<acute>CRB) \<rbrace>) \<longmapsto> ( 
+        \<lbrace> CleanQ_RB_deq_y_P \<acute>uni \<acute>CRB (CleanQ_RB_read_tail_y \<acute>CRB) \<rbrace>
+        \<acute>buf_y := (CleanQ_RB_read_tail_y \<acute>CRB) ;;
+        \<lbrace> CleanQ_RB_deq_y_Q \<acute>uni \<acute>CRB \<acute>buf_y \<rbrace>
+        \<acute>CRB := (CleanQ_RB_incr_tail_y \<acute>buf_y \<acute>CRB) ;;
+        \<lbrace> CleanQ_RB_deq_y_R \<acute>uni \<acute>CRB \<acute>buf_y \<rbrace>
+        SKIP)
+    OD
+    \<lbrace>  CleanQ_RB_Invariants \<acute>uni \<acute>CRB \<rbrace>, \<lbrace>True\<rbrace>
+  COEND
+  \<lbrace>  CleanQ_RB_Invariants \<acute>uni \<acute>CRB \<rbrace>, \<lbrace>True\<rbrace>" 
   by(oghoare, auto)
 
 
+
+(* ------------------------------------------------------------------------------------ *)
+subsubsection \<open>Concurrency with Atomic Ring Updates\<close>
+(* ------------------------------------------------------------------------------------ *)
 
 lemma CleanQ_RB_concurrent_if_all:
      "\<Gamma>, \<Theta> |\<turnstile>\<^bsub>/{True}\<^esub>   
@@ -4493,16 +4938,12 @@ lemma CleanQ_RB_concurrent_if_all:
     
 
 
-(* ------------------------------------------------------------------------------------ *)
-subsubsection \<open>Helper lemmas specifically for last concurrency proof\<close>
-(* ------------------------------------------------------------------------------------ *)
-
 
 (* ------------------------------------------------------------------------------------ *)
-subsubsection \<open>Final concurrency proof\<close>
+subsubsection \<open>Concurrency with Separated Ring Updates\<close>
 (* ------------------------------------------------------------------------------------ *)
 
-lemma CleanQ_RB_conc_mult_if_all:
+lemma CleanQ_RB_conc_mult_ring_updates:
      "\<Gamma>, \<Theta> |\<turnstile>\<^bsub>/{True}\<^esub>   
       COBEGIN
          \<lbrace>  CleanQ_RB_Invariants \<acute>uni \<acute>CRB \<rbrace>
@@ -4522,12 +4963,288 @@ lemma CleanQ_RB_conc_mult_if_all:
          \<lbrace>  CleanQ_RB_Invariants \<acute>uni \<acute>CRB \<rbrace>, \<lbrace>True\<rbrace>
       COEND
       \<lbrace>  CleanQ_RB_Invariants \<acute>uni \<acute>CRB \<rbrace>, \<lbrace>True\<rbrace>" 
-  apply(oghoare) (* 906 subgoals. Auto after this takes really really long*)
+  apply(oghoare) (* 1162 subgoals. Auto after this takes really really long*)
   apply(auto)[200]
   apply(auto)[100]
   apply(auto)[200]
   apply(auto)[200]
+  apply(auto)[200]
+  apply(auto)[200]
   apply(auto)
   done
+
+(* ------------------------------------------------------------------------------------ *)
+subsubsection \<open>Separated Enq/Deq Conditionals\<close>
+(* ------------------------------------------------------------------------------------ *)
+
+
+
+
+lemma CleanQ_RB_write_head_flags_x_head_rx_y_unchanged:
+  "CleanQ_RB_read_head_rx_y (CleanQ_RB_write_head_flags_x b rb) 
+      = CleanQ_RB_read_head_rx_y rb"
+  unfolding CleanQ_RB_read_head_rx_y_def CleanQ_RB_write_head_flags_x_def 
+  by (simp add: rb_write_head_def)
+
+lemma CleanQ_RB_write_head_region_x_head_rx_y_unchanged:
+  "CleanQ_RB_read_head_rx_y (CleanQ_RB_write_head_region_x b rb) 
+      = CleanQ_RB_read_head_rx_y rb"
+  unfolding CleanQ_RB_read_head_rx_y_def CleanQ_RB_write_head_region_x_def 
+  by (simp add: rb_write_head_def)
+
+lemma CleanQ_RB_write_head_offset_x_head_rx_y_unchanged:
+  "CleanQ_RB_read_head_rx_y (CleanQ_RB_write_head_offset_x b rb) 
+      = CleanQ_RB_read_head_rx_y rb"
+  unfolding CleanQ_RB_read_head_rx_y_def CleanQ_RB_write_head_offset_x_def 
+  by (simp add: rb_write_head_def)
+
+lemma CleanQ_RB_write_head_length_x_head_rx_y_unchanged:
+  "CleanQ_RB_read_head_rx_y (CleanQ_RB_write_head_length_x b rb) 
+      = CleanQ_RB_read_head_rx_y rb"
+  unfolding CleanQ_RB_read_head_rx_y_def CleanQ_RB_write_head_length_x_def 
+  by (simp add: rb_write_head_def)
+
+lemma CleanQ_RB_write_head_valid_length_x_head_rx_y_unchanged:
+  "CleanQ_RB_read_head_rx_y (CleanQ_RB_write_head_valid_length_x b rb) 
+      = CleanQ_RB_read_head_rx_y rb"
+  unfolding CleanQ_RB_read_head_rx_y_def CleanQ_RB_write_head_valid_length_x_def 
+  by (simp add: rb_write_head_def)
+
+lemma CleanQ_RB_write_head_valid_offset_x_head_rx_y_unchanged:
+  "CleanQ_RB_read_head_rx_y (CleanQ_RB_write_head_valid_offset_x b rb) 
+      = CleanQ_RB_read_head_rx_y rb"
+  unfolding CleanQ_RB_read_head_rx_y_def CleanQ_RB_write_head_valid_offset_x_def 
+  by (simp add: rb_write_head_def)
+
+lemmas CleanQ_RB_write_head_x_head_rx_y_unchanged[simp] = 
+   CleanQ_RB_write_head_flags_x_head_rx_y_unchanged
+   CleanQ_RB_write_head_region_x_head_rx_y_unchanged
+   CleanQ_RB_write_head_offset_x_head_rx_y_unchanged
+   CleanQ_RB_write_head_length_x_head_rx_y_unchanged
+   CleanQ_RB_write_head_valid_length_x_head_rx_y_unchanged
+   CleanQ_RB_write_head_valid_offset_x_head_rx_y_unchanged
+
+
+lemma CleanQ_RB_write_head_flags_y_head_rx_x_unchanged:
+  "CleanQ_RB_read_head_rx_x (CleanQ_RB_write_head_flags_y b rb) 
+      = CleanQ_RB_read_head_rx_x rb"
+  unfolding CleanQ_RB_read_head_rx_x_def CleanQ_RB_write_head_flags_y_def 
+  by (simp add: rb_write_head_def)
+
+lemma CleanQ_RB_write_head_region_y_head_rx_x_unchanged:
+  "CleanQ_RB_read_head_rx_x (CleanQ_RB_write_head_region_y b rb) 
+      = CleanQ_RB_read_head_rx_x rb"
+  unfolding CleanQ_RB_read_head_rx_x_def CleanQ_RB_write_head_region_y_def 
+  by (simp add: rb_write_head_def)
+
+lemma CleanQ_RB_write_head_offset_y_head_rx_x_unchanged:
+  "CleanQ_RB_read_head_rx_x (CleanQ_RB_write_head_offset_y b rb) 
+      = CleanQ_RB_read_head_rx_x rb"
+  unfolding CleanQ_RB_read_head_rx_x_def CleanQ_RB_write_head_offset_y_def 
+  by (simp add: rb_write_head_def)
+
+lemma CleanQ_RB_write_head_length_y_head_rx_x_unchanged:
+  "CleanQ_RB_read_head_rx_x (CleanQ_RB_write_head_length_y b rb) 
+      = CleanQ_RB_read_head_rx_x rb"
+  unfolding CleanQ_RB_read_head_rx_x_def CleanQ_RB_write_head_length_y_def 
+  by (simp add: rb_write_head_def)
+
+lemma CleanQ_RB_write_head_valid_length_y_head_rx_x_unchanged:
+  "CleanQ_RB_read_head_rx_x (CleanQ_RB_write_head_valid_length_y b rb) 
+      = CleanQ_RB_read_head_rx_x rb"
+  unfolding CleanQ_RB_read_head_rx_x_def CleanQ_RB_write_head_valid_length_y_def 
+  by (simp add: rb_write_head_def)
+
+lemma CleanQ_RB_write_head_valid_offset_y_head_rx_x_unchanged:
+  "CleanQ_RB_read_head_rx_x (CleanQ_RB_write_head_valid_offset_y b rb) 
+      = CleanQ_RB_read_head_rx_x rb"
+  unfolding CleanQ_RB_read_head_rx_x_def CleanQ_RB_write_head_valid_offset_y_def 
+  by (simp add: rb_write_head_def)
+
+lemmas CleanQ_RB_write_head_y_head_rx_x_unchanged[simp] = 
+   CleanQ_RB_write_head_flags_y_head_rx_x_unchanged
+   CleanQ_RB_write_head_region_y_head_rx_x_unchanged
+   CleanQ_RB_write_head_offset_y_head_rx_x_unchanged
+   CleanQ_RB_write_head_length_y_head_rx_x_unchanged
+   CleanQ_RB_write_head_valid_length_y_head_rx_x_unchanged
+   CleanQ_RB_write_head_valid_offset_y_head_rx_x_unchanged
+
+
+
+lemma CleanQ_RB_write_head_flags_x_read_tail_rx_y_unchanged:
+  "CleanQ_RB_read_tail_rx_y (CleanQ_RB_write_head_flags_x b rb)
+     = CleanQ_RB_read_tail_rx_y rb"
+  unfolding CleanQ_RB_read_tail_rx_y_def CleanQ_RB_write_head_flags_x_def
+  by (simp add: rb_write_head_def)
+
+lemma CleanQ_RB_write_head_region_x_read_tail_rx_y_unchanged:
+  "CleanQ_RB_read_tail_rx_y (CleanQ_RB_write_head_region_x b rb)
+     = CleanQ_RB_read_tail_rx_y rb"
+  unfolding CleanQ_RB_read_tail_rx_y_def CleanQ_RB_write_head_region_x_def
+  by (simp add: rb_write_head_def)
+
+lemma CleanQ_RB_write_head_offset_x_read_tail_rx_y_unchanged:
+  "CleanQ_RB_read_tail_rx_y (CleanQ_RB_write_head_offset_x b rb)
+     = CleanQ_RB_read_tail_rx_y rb"
+  unfolding CleanQ_RB_read_tail_rx_y_def CleanQ_RB_write_head_offset_x_def
+  by (simp add: rb_write_head_def)
+
+lemma CleanQ_RB_write_head_length_x_read_tail_rx_y_unchanged:
+  "CleanQ_RB_read_tail_rx_y (CleanQ_RB_write_head_length_x b rb)
+     = CleanQ_RB_read_tail_rx_y rb"
+  unfolding CleanQ_RB_read_tail_rx_y_def CleanQ_RB_write_head_length_x_def
+  by (simp add: rb_write_head_def)
+
+lemma CleanQ_RB_write_head_valid_offset_x_read_tail_rx_y_unchanged:
+  "CleanQ_RB_read_tail_rx_y (CleanQ_RB_write_head_valid_offset_x b rb)
+     = CleanQ_RB_read_tail_rx_y rb"
+  unfolding CleanQ_RB_read_tail_rx_y_def CleanQ_RB_write_head_valid_offset_x_def
+  by (simp add: rb_write_head_def)
+
+lemma CleanQ_RB_write_head_valid_length_x_read_tail_rx_y_unchanged:
+  "CleanQ_RB_read_tail_rx_y (CleanQ_RB_write_head_valid_length_x b rb)
+     = CleanQ_RB_read_tail_rx_y rb"
+  unfolding CleanQ_RB_read_tail_rx_y_def CleanQ_RB_write_head_valid_length_x_def
+  by (simp add: rb_write_head_def)
+
+lemmas CleanQ_RB_write_head_x_read_tail_rx_y_unchanged_simps[simp] = 
+      CleanQ_RB_write_head_flags_x_read_tail_rx_y_unchanged
+      CleanQ_RB_write_head_region_x_read_tail_rx_y_unchanged
+      CleanQ_RB_write_head_offset_x_read_tail_rx_y_unchanged
+      CleanQ_RB_write_head_length_x_read_tail_rx_y_unchanged
+      CleanQ_RB_write_head_valid_offset_x_read_tail_rx_y_unchanged
+      CleanQ_RB_write_head_valid_length_x_read_tail_rx_y_unchanged
+
+
+lemma CleanQ_RB_write_head_flags_y_read_tail_rx_x_unchanged:
+  "CleanQ_RB_read_tail_rx_x (CleanQ_RB_write_head_flags_y b rb)
+     = CleanQ_RB_read_tail_rx_x rb"
+  unfolding CleanQ_RB_read_tail_rx_x_def CleanQ_RB_write_head_flags_y_def
+  by (simp add: rb_write_head_def)
+
+lemma CleanQ_RB_write_head_region_y_read_tail_rx_x_unchanged:
+  "CleanQ_RB_read_tail_rx_x (CleanQ_RB_write_head_region_y b rb)
+     = CleanQ_RB_read_tail_rx_x rb"
+  unfolding CleanQ_RB_read_tail_rx_x_def CleanQ_RB_write_head_region_y_def
+  by (simp add: rb_write_head_def)
+
+lemma CleanQ_RB_write_head_offset_y_read_tail_rx_x_unchanged:
+  "CleanQ_RB_read_tail_rx_x (CleanQ_RB_write_head_offset_y b rb)
+     = CleanQ_RB_read_tail_rx_x rb"
+  unfolding CleanQ_RB_read_tail_rx_x_def CleanQ_RB_write_head_offset_y_def
+  by (simp add: rb_write_head_def)
+
+lemma CleanQ_RB_write_head_length_y_read_tail_rx_x_unchanged:
+  "CleanQ_RB_read_tail_rx_x (CleanQ_RB_write_head_length_y b rb)
+     = CleanQ_RB_read_tail_rx_x rb"
+  unfolding CleanQ_RB_read_tail_rx_x_def CleanQ_RB_write_head_length_y_def
+  by (simp add: rb_write_head_def)
+
+lemma CleanQ_RB_write_head_valid_offset_y_read_tail_rx_x_unchanged:
+  "CleanQ_RB_read_tail_rx_x (CleanQ_RB_write_head_valid_offset_y b rb)
+     = CleanQ_RB_read_tail_rx_x rb"
+  unfolding CleanQ_RB_read_tail_rx_x_def CleanQ_RB_write_head_valid_offset_y_def
+  by (simp add: rb_write_head_def)
+
+lemma CleanQ_RB_write_head_valid_length_y_read_tail_rx_x_unchanged:
+  "CleanQ_RB_read_tail_rx_x (CleanQ_RB_write_head_valid_length_y b rb)
+     = CleanQ_RB_read_tail_rx_x rb"
+  unfolding CleanQ_RB_read_tail_rx_x_def CleanQ_RB_write_head_valid_length_y_def
+  by (simp add: rb_write_head_def)
+
+lemmas CleanQ_RB_write_head_y_read_tail_rx_x_unchanged_simps[simp] = 
+      CleanQ_RB_write_head_flags_y_read_tail_rx_x_unchanged
+      CleanQ_RB_write_head_region_y_read_tail_rx_x_unchanged
+      CleanQ_RB_write_head_offset_y_read_tail_rx_x_unchanged
+      CleanQ_RB_write_head_length_y_read_tail_rx_x_unchanged
+      CleanQ_RB_write_head_valid_offset_y_read_tail_rx_x_unchanged
+      CleanQ_RB_write_head_valid_length_y_read_tail_rx_x_unchanged
+
+lemma CleanQ_RB_deq_x_read_head_rx_y:
+  "CleanQ_RB_read_head_rx_y (CleanQ_RB_deq_x rb) = CleanQ_RB_read_head_rx_y rb"
+  by (simp add: CleanQ_RB_deq_x_def CleanQ_RB_read_head_rx_y_def prod.case_eq_if)
+
+lemma CleanQ_RB_deq_y_read_head_rx_x:
+  "CleanQ_RB_read_head_rx_x (CleanQ_RB_deq_y rb) = CleanQ_RB_read_head_rx_x rb"
+  by (simp add: CleanQ_RB_deq_y_def CleanQ_RB_read_head_rx_x_def prod.case_eq_if)
+
+lemma CleanQ_RB_enq_x_read_tail_rx_y:
+  "CleanQ_RB_read_tail_rx_y (CleanQ_RB_enq_x b rb) = CleanQ_RB_read_tail_rx_y rb"
+  by(simp add: CleanQ_RB_enq_x_def CleanQ_RB_read_tail_rx_y_def rb_enq_equiv rb_enq_alt_def)
+
+lemma CleanQ_RB_enq_y_read_tail_rx_x:
+  "CleanQ_RB_read_tail_rx_x (CleanQ_RB_enq_y b rb) = CleanQ_RB_read_tail_rx_x rb"
+  by(simp add: CleanQ_RB_enq_y_def CleanQ_RB_read_tail_rx_x_def rb_enq_equiv rb_enq_alt_def)
+
+lemma CleanQ_RB_deq_y_read_tail_rx_x:
+  "CleanQ_RB_read_tail_rx_x (CleanQ_RB_deq_y rb) = CleanQ_RB_read_tail_rx_x rb"
+  unfolding CleanQ_RB_read_tail_rx_x_def CleanQ_RB_deq_y_def
+  by (simp add: rb_deq_def)
+
+lemma CleanQ_RB_deq_x_read_tail_rx_y:
+  "CleanQ_RB_read_tail_rx_y (CleanQ_RB_deq_x rb) = CleanQ_RB_read_tail_rx_y rb"
+  unfolding CleanQ_RB_read_tail_rx_y_def CleanQ_RB_deq_x_def
+  by (simp add: rb_deq_def)
+
+lemmas CleanQ_RB_enq_deq_read_tail_head_simps[simp] = 
+  CleanQ_RB_deq_x_read_head_rx_y
+  CleanQ_RB_deq_y_read_head_rx_x
+  CleanQ_RB_enq_x_read_tail_rx_y
+  CleanQ_RB_enq_y_read_tail_rx_x
+  CleanQ_RB_deq_y_read_tail_rx_x
+  CleanQ_RB_deq_x_read_tail_rx_y
+
+lemma CleanQ_RB_conc_mult_ring_updates:
+   "\<Gamma>, \<Theta> |\<turnstile>\<^bsub>/{True}\<^esub>   
+    COBEGIN
+       \<lbrace>  CleanQ_RB_Invariants \<acute>uni \<acute>CRB \<rbrace>
+       WHILE True INV \<lbrace>  CleanQ_RB_Invariants \<acute>uni \<acute>CRB \<rbrace>
+       DO  
+          CleanQ_CRB_enq_mult_x b;;
+          CleanQ_CRB_deq_mult_if_x
+       OD
+       \<lbrace>  CleanQ_RB_Invariants \<acute>uni \<acute>CRB \<rbrace>, \<lbrace>True\<rbrace>  
+       \<parallel> 
+       \<lbrace>  CleanQ_RB_Invariants \<acute>uni \<acute>CRB \<rbrace>
+       WHILE True INV \<lbrace>  CleanQ_RB_Invariants \<acute>uni \<acute>CRB \<rbrace>
+       DO 
+          CleanQ_CRB_enq_mult_y b2;;
+          CleanQ_CRB_deq_mult_if_y
+       OD
+       \<lbrace>  CleanQ_RB_Invariants \<acute>uni \<acute>CRB \<rbrace>, \<lbrace>True\<rbrace>
+    COEND
+    \<lbrace>  CleanQ_RB_Invariants \<acute>uni \<acute>CRB \<rbrace>, \<lbrace>True\<rbrace>" 
+  apply(oghoare) (* 1450 subgoals. Auto after this takes really really long*)
+  apply(auto)[100]
+  apply(auto)[100]
+  apply(auto)[100]
+  apply(auto)[100]
+  apply(auto)[100]
+  apply(auto)[100]
+  apply(auto)[100]
+  apply(auto)[100]
+  apply(auto)[100]
+  apply(auto)[100]
+  apply(auto)[100]
+  apply(auto)[100]
+  apply(auto)[100]
+  apply(auto)[100]
+  apply(auto)
+  oops
+
+
+lemma "CleanQ_RB_read_head_rx_x (CRB x) = CleanQ_RB_read_head_rx_x (CleanQ_RB_enq_y b (CRB x))"
+  oops
+
+lemma "CleanQ_RB_read_head_rx_y (CRB x) = CleanQ_RB_read_head_rx_y (CleanQ_RB_enq_x b (CRB x))"
+  oops
+
+
+
+(* ------------------------------------------------------------------------------------ *)
+subsubsection \<open>Final Concurrency Proofs\<close>
+(* ------------------------------------------------------------------------------------ *)
+
+
 
 end 
